Adjusted Spanning_Trees to reflect changes in Matroids_Greedy

Spanning_Trees/Kruskal_Greedy2.thy
@@ -1,6 +1,6 @@
 theory Kruskal_Greedy2
   imports Matroids_Greedy.Best_In_Greedy Spanning_Trees Encoding
-         Graph_Algorithms.DFS_Example Insertion_Sort_Desc "HOL-Library.Product_Lexorder"
+    Graph_Algorithms_Dev.DFS_Example Insertion_Sort_Desc "HOL-Library.Product_Lexorder"
 begin
 
 hide_const RBT_Set.insert
@@ -21,20 +21,6 @@ lemma tree_split_case:
   "(case t of Leaf \<Rightarrow> True | _ \<Rightarrow> False) = (t = Leaf)"
   by (fastforce split: tree.splits) 
 
-fun rbt_subseteq :: "('a::linorder) rbt \<Rightarrow> 'a rbt \<Rightarrow> bool" where
-  "rbt_subseteq t1 t2 = (case (RBT.diff t1 t2) of Leaf \<Rightarrow> True | _ \<Rightarrow> False)"
-
-lemma rbt_subseteq_correct:
-  "vset_inv t1 \<Longrightarrow> vset_inv t2 \<Longrightarrow> (rbt_subseteq t1 t2) = (Tree2.set_tree t1 \<subseteq> Tree2.set_tree t2)"
-proof(unfold rbt_subseteq.simps tree.split[of "\<lambda> x. x= (_ \<subseteq> _)" True "\<lambda> _ _ _. False" "RBT.diff t1 t2" ],
-      goal_cases)
-  case 1
-  have is_empty_iff:"RBT.diff t1 t2 = \<langle>\<rangle> \<longleftrightarrow> Tree2.set_tree t1 - Tree2.set_tree t2 = {}"
-    using 1  Tree2.eq_set_tree_empty  RBT.set_tree_diff[of t1 t2, symmetric]
-    by (simp add: vset_inv_def)
-  show ?case 
-    using is_empty_iff by (subst Diff_eq_empty_iff[symmetric])fastforce
-qed
 
 lemma rbt_size_correct:
   "vset_inv X \<Longrightarrow> size X = card (Tree2.set_tree X)"
@@ -55,52 +41,50 @@ next
     using 2(3) bst.simps(2)[simplified Tree2.set_inorder[symmetric]] 
     by (metis not_less_iff_gr_or_eq vset_inv_def)
   show ?case 
-   using a_not_down inter_empty 
-   by(auto  simp add: card_Un_disjoint card_insert_if  2(1)[OF vset_inv_l] 2(2)[OF vset_inv_r])
+    using a_not_down inter_empty 
+    by(auto  simp add: card_Un_disjoint card_insert_if  2(1)[OF vset_inv_l] 2(2)[OF vset_inv_r])
 qed
 
-interpretation Custom_Set_RBT: Custom_Set
+lemma rbt_nonempty_repr:
+  "vset_inv X \<Longrightarrow> X \<noteq> \<langle>\<rangle> \<Longrightarrow> Tree2.set_tree X \<noteq> Tree2.set_tree \<langle>\<rangle>"
+  by auto
+
+global_interpretation Card_Set2_RBT: Card_Set2
   where empty = "\<langle>\<rangle>" and insert = insert_rbt and delete = delete_rbt and invar = "vset_inv::(('e::linorder) rbt \<Rightarrow> bool)" and
     isin = isin and set = "Tree2.set_tree" and union = "RBT.union" and inter = "RBT.inter" and diff = "RBT.diff" and
-    subseteq = rbt_subseteq and cardinality = size
-  apply (subst Custom_Set_def)
+    cardinality = size
+  defines subseteq = Card_Set2_RBT.subseteq
+  apply (subst Card_Set2_def)
   apply(intro conjI)
   subgoal
     using RBT.Set2_axioms
     by (metis RBT_Set.empty_def dfs.set_ops.Set2_axioms)
   subgoal
-    apply (subst Custom_Set_axioms_def)
-    using rbt_subseteq_correct rbt_size_correct by blast
+    apply (subst Card_Set2_axioms_def)
+    using rbt_nonempty_repr rbt_size_correct by blast
   done
-
-
-definition "set_of_sets_isin f a = f a"
-
-lemma set_of_sets_isin_def': "set_of_sets_isin = id"
-  using set_of_sets_isin_def by fastforce
 
 interpretation Matroid_Specs_Inst: Matroid_Specs
   where set_empty = "\<langle>\<rangle>" and set_insert = insert_rbt and set_delete = delete_rbt and set_inv = "vset_inv::(('e::linorder) rbt \<Rightarrow> bool)" and
     set_isin = isin and to_set = "Tree2.set_tree" and union = "RBT.union" and inter = "RBT.inter" and diff = "RBT.diff" and
-    subseteq = rbt_subseteq and cardinality = size and
-    set_of_sets_isin = "set_of_sets_isin :: ('e rbt \<Rightarrow> bool) \<Rightarrow> 'e rbt \<Rightarrow> bool"
+    cardinality = size 
   apply (subst Matroid_Specs_def)
   apply (subst Indep_System_Specs_def)
-  using Custom_Set_RBT.Custom_Set_axioms by blast
+  using Card_Set2_RBT.Card_Set2_axioms by blast
 
 fun rbt_set_fold :: "'a rbt \<Rightarrow> ('a \<Rightarrow> 'b \<Rightarrow> 'b) \<Rightarrow> 'b \<Rightarrow> 'b" where
   "rbt_set_fold Leaf f acc = acc"
 | "rbt_set_fold (Node l (a, _) r) f acc = rbt_set_fold r f (f a (rbt_set_fold l f acc))"
 
 lemma rbt_set_fold_revinorder: "rbt_set_fold T f acc = foldr f (rev (inorder T)) acc"
- by(induction T f acc rule: rbt_set_fold.induct) auto
+  by(induction T f acc rule: rbt_set_fold.induct) auto
 
 fun rbt_map_fold :: "('a \<times> 'd) rbt \<Rightarrow> ('a \<Rightarrow> 'd \<Rightarrow> 'b \<Rightarrow> 'b) \<Rightarrow> 'b \<Rightarrow> 'b" where
   "rbt_map_fold Leaf f acc = acc"
 | "rbt_map_fold (Node l ((a, d), _) r) f acc = rbt_map_fold r f (f a d (rbt_map_fold l f acc))"
 
 lemma rbt_map_fold_revinorder: "rbt_map_fold T f acc = foldr (\<lambda> (x, y) acc. f x y acc) (rev (inorder T)) acc"
- by(induction T f acc rule: rbt_map_fold.induct) auto
+  by(induction T f acc rule: rbt_map_fold.induct) auto
 
 global_interpretation Kruskal_Graphs_Matroids: Encoding
   where empty = RBT_Set.empty and update = update and delete = RBT_Map.delete and
@@ -108,16 +92,15 @@ global_interpretation Kruskal_Graphs_Matroids: Encoding
     insert = insert_rbt and vset_delete = delete_rbt and vset_inv = "vset_inv::(('v::linorder) rbt \<Rightarrow> bool)" and
     isin = isin and t_set = "Tree2.set_tree" and sel = sel and
 
-    set_empty = "\<langle>\<rangle>" and set_insert = insert_rbt and set_delete = delete_rbt and set_inv = "vset_inv::(('e::linorder) rbt \<Rightarrow> bool)" and
-    set_isin = isin and to_set = "Tree2.set_tree" and union = "RBT.union" and inter = "RBT.inter" and diff = "RBT.diff" and
-    adjmap_fold = "rbt_map_fold" and vset_fold = "rbt_set_fold" and set_fold_adjmap = "rbt_set_fold" and
-    set_fold_vset = "rbt_set_fold"
-    for v1_of :: "('e::linorder) \<Rightarrow> ('v::linorder)" and v2_of :: "('e::linorder) \<Rightarrow> ('v::linorder)" (*and 
-        edge_of :: "('v::linorder) \<Rightarrow> 'v \<Rightarrow> ('e::linorder)"*) and c :: "('v set) \<Rightarrow> rat" and c' :: "'e \<Rightarrow> rat"
-      defines (*graph_to_edges = Kruskal_Graphs_Matroids.graph_to_edges
-and*) edges_to_graph = Kruskal_Graphs_Matroids.edges_to_graph
-and edges_to_vertices = Kruskal_Graphs_Matroids.edges_to_vertices
-  by (auto intro: Encoding.intro simp add: Custom_Set_RBT.Set2_axioms Pair_Graph_U_RBT.Pair_Graph_U_Specs_axioms)
+set_empty = "\<langle>\<rangle>" and set_insert = insert_rbt and set_delete = delete_rbt and set_inv = "vset_inv::(('e::linorder) rbt \<Rightarrow> bool)" and
+set_isin = isin and to_set = "Tree2.set_tree" and union = "RBT.union" and inter = "RBT.inter" and diff = "RBT.diff" and
+adjmap_fold = "rbt_map_fold" and vset_fold = "rbt_set_fold" and set_fold_adjmap = "rbt_set_fold" and
+set_fold_vset = "rbt_set_fold"
+for v1_of :: "('e::linorder) \<Rightarrow> ('v::linorder)" and v2_of :: "('e::linorder) \<Rightarrow> ('v::linorder)" 
+  and c :: "('v set) \<Rightarrow> rat" and c' :: "'e \<Rightarrow> rat"
+defines edges_to_graph = Kruskal_Graphs_Matroids.edges_to_graph
+  and edges_to_vertices = Kruskal_Graphs_Matroids.edges_to_vertices
+  by (auto intro: Encoding.intro simp add: Card_Set2_RBT.Set2_axioms Pair_Graph_U_RBT.Pair_Graph_U_Specs_axioms)
 
 
 
@@ -145,7 +128,7 @@ lemma  rbt_map_fold_correct: "M.invar G \<Longrightarrow>
 proof(subst rbt_map_fold_revinorder, rule exI[of _ "map fst (rev (inorder G))"], goal_cases)
   case 1
   have invar_inorder:"rbt G \<and> sorted1 (Tree2.inorder G)"
-   using "1" M.invar_def by auto
+    using "1" M.invar_def by auto
   define list where "list = Tree2.inorder G"
   define list' where "list' = rev (inorder G)"
   have distinct_list:"distinct (map fst (Tree2.inorder G))" 
@@ -198,11 +181,11 @@ proof(subst rbt_map_fold_revinorder, rule exI[of _ "map fst (rev (inorder G))"],
       qed
     qed
     show ?thesis
-    using invar_inorder 
-    by(simp add:  lookup_map_of map_of_rev[OF distinct_list, symmetric] list'_def[symmetric] same_fold)+  
+      using invar_inorder 
+      by(simp add:  lookup_map_of map_of_rev[OF distinct_list, symmetric] list'_def[symmetric] same_fold)+  
   qed
- ultimately show ?case 
-   by (metis distinct_rev rev_map set_rev)
+  ultimately show ?case 
+    by (metis distinct_rev rev_map set_rev)
 qed
 
 lemma bst_distinct_inorder:"bst T \<Longrightarrow> distinct (inorder T)"
@@ -214,9 +197,9 @@ lemma rbt_set_fold_correct: "vset_inv S \<Longrightarrow> \<exists>xs. distinct 
   using  bst_distinct_inorder[of S]
   by(unfold set_inorder[symmetric] set_rev distinct_rev)(simp add: vset_inv_def )
 
-locale Transforms =
-fixes v1_of::"('e::linorder \<Rightarrow> 'v::linorder)" and v2_of::"'e \<Rightarrow> 'v" 
-and input_G :: "'e rbt"
+locale Oracle =
+  fixes v1_of::"('e::linorder \<Rightarrow> 'v::linorder)" and v2_of::"'e \<Rightarrow> 'v" 
+    and input_G :: "'e rbt"
 begin
 
 definition Kruskal_E_to_G :: "('e::linorder) rbt \<Rightarrow> ('v \<times> ('v rbt)) rbt" where
@@ -230,36 +213,35 @@ definition indep_graph_matroid :: "('e::linorder) rbt \<Rightarrow> bool" where
                               (Tree2.set_tree input_G) (Tree2.set_tree E))"
 
 definition "local_indep_oracle e X = 
-((rbt_subseteq (vset_insert e X) input_G) \<and>
+((Card_Set2_RBT.subseteq (vset_insert e X) input_G) \<and>
                    (lookup (Kruskal_E_to_G X) (v2_of e) \<noteq> None \<and> lookup (Kruskal_E_to_G X) (v1_of e) \<noteq> None\<longrightarrow>
                    return (dfs_impl (Kruskal_E_to_G X) (v2_of e) (dfs_initial_state (v1_of e))) 
                     = NotReachable))"
 
 end
 
-global_interpretation transforms: Transforms
+global_interpretation orcl: Oracle
   where v1_of = v1_of and v2_of = v2_of  and input_G = input_G
   for v1_of::"'e::linorder \<Rightarrow> 'a::linorder" and v2_of edge_of input_G
-  defines Kruskal_E_to_G=transforms.Kruskal_E_to_G
-   and Kruskal_E_to_V=transforms.Kruskal_E_to_V
-   and indep_graph_matroid=transforms.indep_graph_matroid
-   and local_indep_oracle= transforms.local_indep_oracle
+  defines Kruskal_E_to_G=orcl.Kruskal_E_to_G
+    and Kruskal_E_to_V=orcl.Kruskal_E_to_V
+    and indep_graph_matroid=orcl.indep_graph_matroid
+    and local_indep_oracle= orcl.local_indep_oracle
   done
 
 global_interpretation Kruskal_Greedy: Best_In_Greedy'
   where set_empty = "\<langle>\<rangle>" and set_insert = insert_rbt and set_delete = delete_rbt 
-     and set_inv = "vset_inv::(('e::linorder) rbt \<Rightarrow> bool)" and
+    and set_inv = "vset_inv::(('e::linorder) rbt \<Rightarrow> bool)" and
     set_isin = isin and to_set = "Tree2.set_tree" and union = "RBT.union" and inter = "RBT.inter" and diff = "RBT.diff" and
-    subseteq = rbt_subseteq and cardinality = size and
-    set_of_sets_isin = "set_of_sets_isin :: (('e::linorder) rbt \<Rightarrow> bool) \<Rightarrow> 'e rbt \<Rightarrow> bool" and 
+    cardinality = size and
     carrier = input_G and 
-    indep_set = "indep_graph_matroid v1_of v2_of input_G" and
+    indep_fn = "indep_graph_matroid v1_of v2_of input_G" and
     sort_desc = insort_key_desc and 
     local_indep_oracle = "local_indep_oracle v1_of v2_of input_G"
     and wrapper_insert = insert_rbt
-and wrapper_invar = "vset_inv::(('e::linorder) rbt \<Rightarrow> bool)"
-and remove_wrapper = id
-and wrapper_empty = Leaf
+    and wrapper_invar = "vset_inv::(('e::linorder) rbt \<Rightarrow> bool)"
+    and remove_wrapper = id
+    and wrapper_empty = Leaf
   for v1_of::"'e::linorder \<Rightarrow>'a::linorder" and v2_of input_G
   defines kruskal' = Kruskal_Greedy.BestInGreedy'
     and  kruskal = Kruskal_Greedy.BestInGreedy
@@ -268,12 +250,12 @@ and wrapper_empty = Leaf
     and indep' = "Kruskal_Greedy.indep'"
     and to_ordinary = Kruskal_Greedy.to_ordinary
   apply (subst Best_In_Greedy'_def, subst Best_In_Greedy_def)
- by(auto intro!: Best_In_Greedy'_axioms.intro 
-simp add: Matroid_Specs_Inst.Matroid_Specs_axioms Pair_Graph_RBT.set.Set_axioms
- dfs.Graph.vset.set.invar_insert set.invar_empty)
+  by(auto intro!: Best_In_Greedy'_axioms.intro 
+      simp add: Matroid_Specs_Inst.Matroid_Specs_axioms Pair_Graph_RBT.set.Set_axioms
+      dfs.Graph.vset.set.invar_insert set.invar_empty)
 
 locale Kruskal_Proof_Matroid_Edges =
-Transforms where v1_of = "v1_of::'e::linorder \<Rightarrow> 'v::linorder" for v1_of+
+  Oracle where v1_of = "v1_of::'e::linorder \<Rightarrow> 'v::linorder" for v1_of+
 assumes v1_never_v2:"\<And> e. v1_of e \<noteq> v2_of e"
 begin
 
@@ -281,7 +263,7 @@ context
   assumes  G_good: "vset_inv input_G"
 begin
 lemma Encoding_Proofs_axioms:
- " Encoding_Proofs_axioms t_set M.invar vset_inv lookup vset_inv t_set rbt_map_fold
+  " Encoding_Proofs_axioms t_set M.invar vset_inv lookup vset_inv t_set rbt_map_fold
      rbt_set_fold rbt_set_fold rbt_set_fold v1_of v2_of"(* edge_of"*)
 proof(rule Encoding_Proofs_axioms.intro, goal_cases)
   case (1 G S f)
@@ -308,7 +290,7 @@ next
   then show ?case 
     by (simp add: v1_never_v2)
 qed
-(*
+  (*
 next
   case (7 x y)
   then show ?case
@@ -325,17 +307,17 @@ interpretation Kruskal_Graphs_Matroids_proofs: Encoding_Proofs
     insert = insert_rbt and vset_delete = delete_rbt and vset_inv = "vset_inv::(('v::linorder) rbt \<Rightarrow> bool)" and
     isin = isin and t_set = "Tree2.set_tree" and sel = sel and
 
-    set_empty = "\<langle>\<rangle>" and set_insert = insert_rbt and set_delete = delete_rbt and set_inv = "vset_inv::(('e::linorder) rbt \<Rightarrow> bool)" and
-    set_isin = isin and to_set = "Tree2.set_tree" and union = "RBT.union" and inter = "RBT.inter" and diff = "RBT.diff" and
-    adjmap_fold = "rbt_map_fold" and vset_fold = "rbt_set_fold" and set_fold_adjmap = "rbt_set_fold" and
-    set_fold_vset = "rbt_set_fold"
-  for c :: "('v set) \<Rightarrow> rat" and c' :: "'e \<Rightarrow> rat"
+set_empty = "\<langle>\<rangle>" and set_insert = insert_rbt and set_delete = delete_rbt and set_inv = "vset_inv::(('e::linorder) rbt \<Rightarrow> bool)" and
+set_isin = isin and to_set = "Tree2.set_tree" and union = "RBT.union" and inter = "RBT.inter" and diff = "RBT.diff" and
+adjmap_fold = "rbt_map_fold" and vset_fold = "rbt_set_fold" and set_fold_adjmap = "rbt_set_fold" and
+set_fold_vset = "rbt_set_fold"
+for c :: "('v set) \<Rightarrow> rat" and c' :: "'e \<Rightarrow> rat"
   by(auto intro!: Encoding_Proofs.intro  Encoding_Proofs_axioms 
-           simp add: Encoding_def 
-            Pair_Graph_U_RBT.Pair_Graph_U_Specs_axioms Custom_Set_RBT.Set2_axioms)
+      simp add: Encoding_def 
+      Pair_Graph_U_RBT.Pair_Graph_U_Specs_axioms Card_Set2_RBT.Set2_axioms)
 
 lemma pair_graph_u_invar:
-"vset_inv S \<Longrightarrow> Pair_Graph_U_RBT.pair_graph_u_invar (Kruskal_E_to_G S)"
+  "vset_inv S \<Longrightarrow> Pair_Graph_U_RBT.pair_graph_u_invar (Kruskal_E_to_G S)"
   by (simp add: Kruskal_Graphs_Matroids_proofs.edges_invar_imp_graph_invar edges_to_graph_def local.Kruskal_E_to_G_def)
 
 lemma same_dgraphabs:"dfs.Graph.digraph_abs = G.digraph_abs"
@@ -350,18 +332,18 @@ interpretation undirected_multigraph: undirected_multigraph to_dbltn "Tree2.set_
 
 lemma local_indep_oracle_correct:
   assumes "vset_inv S"
-        "indep' v1_of v2_of input_G (id S)"
-        "rbt_subseteq (id S) input_G"
-        "e \<notin> t_set (id S)"
- shows "local_indep_oracle e S = indep' v1_of v2_of input_G (vset_insert e (id S))"
+    "indep' v1_of v2_of input_G (id S)"
+    "Card_Set2_RBT.subseteq (id S) input_G"
+    "e \<notin> t_set (id S)"
+  shows "local_indep_oracle e S = indep' v1_of v2_of input_G (vset_insert e (id S))"
   apply(insert assms)
-  unfolding indep'_def Matroid_Specs_Inst.indep_def Kruskal_Greedy2.indep_graph_matroid_def
-            indep_graph_matroid_def set_of_sets_isin_def 
+  unfolding indep'_def Kruskal_Greedy2.indep_graph_matroid_def
+    indep_graph_matroid_def
 proof(goal_cases)
   case 1
   note case_assms = this
-  have first_eq:"rbt_subseteq (vset_insert e S) input_G = (t_set (vset_insert e (id S)) \<subseteq> t_set input_G)" 
-    using G_good assms(1) dfs.Graph.vset.set.invar_insert rbt_subseteq_correct by auto
+  have first_eq:"Card_Set2_RBT.subseteq (vset_insert e S) input_G = (t_set (vset_insert e (id S)) \<subseteq> t_set input_G)" 
+    using G_good assms(1) dfs.Graph.vset.set.invar_insert Card_Set2_RBT.set_subseteq by auto
   have second_eq:"(((lookup (local.Kruskal_E_to_G S) (v2_of e) \<noteq> None \<and> lookup (Kruskal_E_to_G S) (v1_of e) \<noteq> None) \<longrightarrow>
                  (return (dfs_impl (local.Kruskal_E_to_G S) (v2_of e) 
                  (dfs_initial_state (v1_of e))) = NotReachable))) =
@@ -370,372 +352,372 @@ proof(goal_cases)
   proof-
     have digraph_abs_is:"G.digraph_abs (Kruskal_E_to_G S) =
      (\<lambda>e. (v1_of e, v2_of e)) ` t_set S \<union> (\<lambda>e. (v2_of e, v1_of e)) ` t_set S"
-     by(auto intro!: Kruskal_Graphs_Matroids_proofs.digraph_abs_of_edges_of_to_graph_general
-            simp add: assms(1) Kruskal_E_to_G_def edges_to_graph_def )
-   have ugraph_abs_is: "Pair_Graph_U_RBT.ugraph_abs (Kruskal_E_to_G S) = to_dbltn ` (t_set  S)"
-    by(auto intro!: Kruskal_Graphs_Matroids_proofs.dbltn_set_and_ugraph_abs[symmetric]
-            simp add: assms(1) Kruskal_E_to_G_def edges_to_graph_def )
-   have pair_graph_u_invar:"Pair_Graph_U_RBT.pair_graph_u_invar (edges_to_graph  v1_of  v2_of S)" 
-     using assms(1) local.Kruskal_E_to_G_def pair_graph_u_invar by auto
-   have double_ex_I: "rest x y \<Longrightarrow> \<exists>v1 v2.
+      by(auto intro!: Kruskal_Graphs_Matroids_proofs.digraph_abs_of_edges_of_to_graph_general
+          simp add: assms(1) Kruskal_E_to_G_def edges_to_graph_def )
+    have ugraph_abs_is: "Pair_Graph_U_RBT.ugraph_abs (Kruskal_E_to_G S) = to_dbltn ` (t_set  S)"
+      by(auto intro!: Kruskal_Graphs_Matroids_proofs.dbltn_set_and_ugraph_abs[symmetric]
+          simp add: assms(1) Kruskal_E_to_G_def edges_to_graph_def )
+    have pair_graph_u_invar:"Pair_Graph_U_RBT.pair_graph_u_invar (edges_to_graph  v1_of  v2_of S)" 
+      using assms(1) local.Kruskal_E_to_G_def pair_graph_u_invar by auto
+    have double_ex_I: "rest x y \<Longrightarrow> \<exists>v1 v2.
        {x, y} = {v1, v2} \<and> rest v1 v2" for x y rest by auto
-   have lookup_in_dVs:"lookup (local.Kruskal_E_to_G S) x = Some y\<Longrightarrow> 
+    have lookup_in_dVs:"lookup (local.Kruskal_E_to_G S) x = Some y\<Longrightarrow> 
           x \<in> dVs (dfs.Graph.digraph_abs (local.Kruskal_E_to_G S))" for x y
-     using Kruskal_Graphs_Matroids_proofs.edges_invar_imp_graph_invar(2)[OF assms(1)]
-            S_C.choose  
-     by(unfold  dfs.Graph.digraph_abs_def DFS_Example.neighbourhood_def)
-       (auto simp add: Kruskal_E_to_G_def edges_to_graph_def
-                      neighbourhood_def[symmetric] dfs.Graph.neighbourhood_def dVs_def
-               intro!: exI[of _ "{x, sel y}"]  double_ex_I)
-   have "lookup (local.Kruskal_E_to_G S) (v1_of e) = Some y \<Longrightarrow>
+      using Kruskal_Graphs_Matroids_proofs.edges_invar_imp_graph_invar(2)[OF assms(1)]
+        S_C.choose  
+      by(unfold  dfs.Graph.digraph_abs_def DFS_Example.neighbourhood_def)
+        (auto simp add: Kruskal_E_to_G_def edges_to_graph_def
+          neighbourhood_def[symmetric] dfs.Graph.neighbourhood_def dVs_def
+          intro!: exI[of _ "{x, sel y}"]  double_ex_I)
+    have "lookup (local.Kruskal_E_to_G S) (v1_of e) = Some y \<Longrightarrow>
          DFS.DFS_axioms isin t_set adj_inv vset_empty vset_inv lookup
           (local.Kruskal_E_to_G S) (v1_of e)" for y
-     unfolding DFS.DFS_axioms_def[OF dfs.DFS_axioms]
-     using   lookup_in_dVs pair_graph_u_invar
-     by(unfold Pair_Graph_U_RBT.pair_graph_u_invar_def Kruskal_E_to_G_def adj_inv_def)
-     simp
-   hence DFS_thms: "lookup (local.Kruskal_E_to_G S) (v1_of e) \<noteq> None \<Longrightarrow>
+      unfolding DFS.DFS_axioms_def[OF dfs.DFS_axioms]
+      using   lookup_in_dVs pair_graph_u_invar
+      by(unfold Pair_Graph_U_RBT.pair_graph_u_invar_def Kruskal_E_to_G_def adj_inv_def)
+        simp
+    hence DFS_thms: "lookup (local.Kruskal_E_to_G S) (v1_of e) \<noteq> None \<Longrightarrow>
         DFS_thms map_empty RBT_Map.delete vset_insert isin t_set sel update adj_inv vset_empty vset_delete vset_inv
      vset_union vset_inter vset_diff lookup (Kruskal_E_to_G S) (v1_of e)"
-     by(auto intro!: DFS_thms.intro dfs.DFS_axioms DFS_thms_axioms.intro )
-   have graph_abs_with_e: "graph_abs (to_dbltn ` insert e (t_set S))"
-     using v1_never_v2 by (auto simp add: graph_abs_def dblton_graph_def Vs_def)
-   have graph_abs_without_e: "graph_abs (to_dbltn `(t_set S))"
-     using graph_abs_mono graph_abs_with_e by auto
-   have graph_abs_vset_insert:"graph_abs (to_dbltn ` t_set (vset_insert e S))"
-     using RBT.set_tree_insert[of S] case_assms(1) graph_abs_with_e 
-     by(simp add:vset_inv_def)
-   show ?thesis 
-     unfolding dfs_impl_def dfs_initial_state_def
-   proof(cases "lookup (local.Kruskal_E_to_G S) (v1_of e) \<noteq> None 
+      by(auto intro!: DFS_thms.intro dfs.DFS_axioms DFS_thms_axioms.intro )
+    have graph_abs_with_e: "graph_abs (to_dbltn ` insert e (t_set S))"
+      using v1_never_v2 by (auto simp add: graph_abs_def dblton_graph_def Vs_def)
+    have graph_abs_without_e: "graph_abs (to_dbltn `(t_set S))"
+      using graph_abs_mono graph_abs_with_e by auto
+    have graph_abs_vset_insert:"graph_abs (to_dbltn ` t_set (vset_insert e S))"
+      using RBT.set_tree_insert[of S] case_assms(1) graph_abs_with_e 
+      by(simp add:vset_inv_def)
+    show ?thesis 
+      unfolding dfs_impl_def dfs_initial_state_def
+    proof(cases "lookup (local.Kruskal_E_to_G S) (v1_of e) \<noteq> None 
          \<and> lookup (local.Kruskal_E_to_G S) (v2_of e) \<noteq> None", goal_cases)
-     case 1
-     hence 1: "lookup (local.Kruskal_E_to_G S) (v1_of e) \<noteq> None" 
-              "lookup (local.Kruskal_E_to_G S) (v2_of e) \<noteq> None" by auto
-     note one = this
-     show ?case
-     proof(subst DFS_thms.DFS_to_DFS_impl[OF DFS_thms, symmetric, OF 1(1)], rule, all \<open>rule ccontr\<close>, goal_cases)
-       case 1
-       then obtain u C where uC_prop:"undirected_multigraph_spec.decycle_multi to_dbltn
-                 (t_set (vset_insert e S)) u C" by auto
-       moreover have  not_cycle_old:"\<not> undirected_multigraph_spec.decycle_multi to_dbltn
-                 (t_set S) u C" 
-         using case_assms(2) 
-         by(simp add: id_def undirected_multigraph_spec.has_no_cycle_multi_def)
-       ultimately have e_and_C:"e \<in> set C" "set C \<subseteq> (t_set (vset_insert e S))"
-         unfolding undirected_multigraph_spec.decycle_multi_def     
-        using epath_subset_other_set[of "insert {v1_of e, v2_of e} (to_dbltn ` t_set S)"
-                                    u "map _ C" u , simplified list.set_map,OF _ image_mono] 
-        by (auto simp add: Pair_Graph_RBT.set.set_insert[OF case_assms(1)])
-      then obtain C1 C2 where C_split:"C = C1@[e]@C2"
-        by (metis append_Cons append_self_conv2 split_list_last)
-      obtain q where q_prop:"walk_betw (to_dbltn ` (insert e (t_set S))) u q u" "map to_dbltn C = edges_of_path q"
-        using graph_abs.epath_imp_walk_betw[of _ u "map to_dbltn C" u, OF graph_abs_with_e] 
-              uC_prop 
-         by(auto simp add: undirected_multigraph_spec.decycle_multi_def  Pair_Graph_RBT.set.set_insert[OF case_assms(1)])
-      
-       hence e_in_p: "to_dbltn e \<in> set (edges_of_path q)"
-        by (metis (mono_tags, lifting) \<open>e \<in> set C\<close> image_set rev_image_eqI)
-      have lengthq: "length q \<ge> 2" 
-        using \<open>to_dbltn e \<in> set (edges_of_path q)\<close> edges_of_path_nempty by fastforce
-      have v1v2: "v1_of e \<noteq> v2_of e" 
-        by (simp add: v1_never_v2)
-    show ?case proof(cases "lookup (local.Kruskal_E_to_G S) (v2_of e)")
-      case None
-       thus ?thesis 
-        by (simp add: one(2))
-    next
-      case (Some neighb)
-      have "\<exists>q. walk_betw (to_dbltn ` t_set (vset_insert e S)) u q u \<and> map to_dbltn C = edges_of_path q"
-        using graph_abs_vset_insert  uC_prop 
-        by(auto intro:graph_abs.epath_imp_walk_betw simp add: undirected_multigraph.decycle_multi_def)
-      have no_distinct_path:"\<nexists>p. distinct p \<and>
-              vwalk_bet (dfs.Graph.digraph_abs (local.Kruskal_E_to_G S)) (v1_of e) p (v2_of e)"
-        using DFS_thms.DFS_correct_1[OF DFS_thms] Some  one 1 by blast
-      have no_other_e:"(to_dbltn e) \<notin> (to_dbltn ` t_set S)"
-      proof(rule, rule ccontr, goal_cases)
+      case 1
+      hence 1: "lookup (local.Kruskal_E_to_G S) (v1_of e) \<noteq> None" 
+        "lookup (local.Kruskal_E_to_G S) (v2_of e) \<noteq> None" by auto
+      note one = this
+      show ?case
+      proof(subst DFS_thms.DFS_to_DFS_impl[OF DFS_thms, symmetric, OF 1(1)], rule, all \<open>rule ccontr\<close>, goal_cases)
         case 1
-        then obtain d where d_prop:"to_dbltn d = to_dbltn e" "d \<in> t_set S" by auto
-        hence "{(v1_of d, v2_of d), (v2_of d, v1_of d)} \<subseteq> (dfs.Graph.digraph_abs (local.Kruskal_E_to_G S))"
-          by (simp add: RBT_Set.empty_def digraph_abs_is)
-        moreover have "(v1_of e, v2_of e) = (v1_of d, v2_of d)\<or>(v1_of e, v2_of e) = (v2_of d, v1_of d)"
-          using d_prop by(unfold doubleton_eq_iff) presburger
-        ultimately have "vwalk_bet (dfs.Graph.digraph_abs (Kruskal_E_to_G S)) 
+        then obtain u C where uC_prop:"undirected_multigraph_spec.decycle_multi to_dbltn
+                 (t_set (vset_insert e S)) u C" by auto
+        moreover have  not_cycle_old:"\<not> undirected_multigraph_spec.decycle_multi to_dbltn
+                 (t_set S) u C" 
+          using case_assms(2) 
+          by(simp add: id_def undirected_multigraph_spec.has_no_cycle_multi_def)
+        ultimately have e_and_C:"e \<in> set C" "set C \<subseteq> (t_set (vset_insert e S))"
+          unfolding undirected_multigraph_spec.decycle_multi_def     
+          using epath_subset_other_set[of "insert {v1_of e, v2_of e} (to_dbltn ` t_set S)"
+              u "map _ C" u , simplified list.set_map,OF _ image_mono] 
+          by (auto simp add: Pair_Graph_RBT.set.set_insert[OF case_assms(1)])
+        then obtain C1 C2 where C_split:"C = C1@[e]@C2"
+          by (metis append_Cons append_self_conv2 split_list_last)
+        obtain q where q_prop:"walk_betw (to_dbltn ` (insert e (t_set S))) u q u" "map to_dbltn C = edges_of_path q"
+          using graph_abs.epath_imp_walk_betw[of _ u "map to_dbltn C" u, OF graph_abs_with_e] 
+            uC_prop 
+          by(auto simp add: undirected_multigraph_spec.decycle_multi_def  Pair_Graph_RBT.set.set_insert[OF case_assms(1)])
+
+        hence e_in_p: "to_dbltn e \<in> set (edges_of_path q)"
+          by (metis (mono_tags, lifting) \<open>e \<in> set C\<close> image_set rev_image_eqI)
+        have lengthq: "length q \<ge> 2" 
+          using \<open>to_dbltn e \<in> set (edges_of_path q)\<close> edges_of_path_nempty by fastforce
+        have v1v2: "v1_of e \<noteq> v2_of e" 
+          by (simp add: v1_never_v2)
+        show ?case proof(cases "lookup (local.Kruskal_E_to_G S) (v2_of e)")
+          case None
+          thus ?thesis 
+            by (simp add: one(2))
+        next
+          case (Some neighb)
+          have "\<exists>q. walk_betw (to_dbltn ` t_set (vset_insert e S)) u q u \<and> map to_dbltn C = edges_of_path q"
+            using graph_abs_vset_insert  uC_prop 
+            by(auto intro:graph_abs.epath_imp_walk_betw simp add: undirected_multigraph.decycle_multi_def)
+          have no_distinct_path:"\<nexists>p. distinct p \<and>
+              vwalk_bet (dfs.Graph.digraph_abs (local.Kruskal_E_to_G S)) (v1_of e) p (v2_of e)"
+            using DFS_thms.DFS_correct_1[OF DFS_thms] Some  one 1 by blast
+          have no_other_e:"(to_dbltn e) \<notin> (to_dbltn ` t_set S)"
+          proof(rule, rule ccontr, goal_cases)
+            case 1
+            then obtain d where d_prop:"to_dbltn d = to_dbltn e" "d \<in> t_set S" by auto
+            hence "{(v1_of d, v2_of d), (v2_of d, v1_of d)} \<subseteq> (dfs.Graph.digraph_abs (local.Kruskal_E_to_G S))"
+              by (simp add: RBT_Set.empty_def digraph_abs_is)
+            moreover have "(v1_of e, v2_of e) = (v1_of d, v2_of d)\<or>(v1_of e, v2_of e) = (v2_of d, v1_of d)"
+              using d_prop by(unfold doubleton_eq_iff) presburger
+            ultimately have "vwalk_bet (dfs.Graph.digraph_abs (Kruskal_E_to_G S)) 
                          (v1_of e) [v1_of e, v2_of e] (v2_of e)" 
-          by fastforce
-        moreover have "distinct [v1_of e, v2_of e]"
-          using v1v2 by auto
-        ultimately show ?case 
-          using   no_distinct_path by blast
-      qed 
-      moreover have dbltn_inj:"inj_on to_dbltn (t_set S) "
-        using case_assms(2) undirected_multigraph.has_no_cycle_multi_to_dbltn_inj by simp
-      ultimately have dbltn_inj_big:"inj_on to_dbltn (insert e (t_set S))" by auto
-      moreover have C_subset:"set C \<subseteq> (insert e (t_set S))"
-        using case_assms(1) dfs.Graph.vset.set.set_insert e_and_C(2) by auto
-      ultimately have inj_C:"inj_on to_dbltn (set C)" 
-        by (meson inj_on_subset)
-      have distinct_edges_q:"distinct (edges_of_path q)"
-        using q_prop(2) distinct_map[of to_dbltn C] uC_prop e_and_C inj_C
-        by(auto simp add: undirected_multigraph.decycle_multi_def) 
-      have e_vs_in_new_v_set:"{v1_of e, v2_of e} \<subseteq> Vs (to_dbltn ` insert e (t_set S))"
-        by (simp add: vs_member)
-      then obtain q1 q2 where q1_q2_prop: "q = q1@[v1_of e, v2_of e]@ q2 \<or> q = q1@[v2_of e, v1_of e]@ q2"
-        using undirected_multigraph.edges_to_path_split_by_edge[of _ _ "v1_of e" "v2_of e"] e_in_p by fast
-       obtain q' where  path_without_e:"walk_betw (to_dbltn `  (t_set S)) (v1_of e) q' (v2_of e)"
-       proof(cases rule: disjE[OF q1_q2_prop], all "cases q1", all \<open>cases q2\<close>, goal_cases)
-         case 1
-         then show ?case 
-           using q_prop(1) v1v2 walk_between_nonempty_pathD(3) walk_between_nonempty_pathD(4) by fastforce
-       next
-         case (2 a list)
-         hence a1:"walk_betw (to_dbltn ` insert e (t_set S)) u (q1 @ [v1_of e]) (v1_of e)"
-           using q_prop(1) by (intro walk_pref[of _ u q1 "v1_of e" "v2_of e # q2" u]) force
-         moreover have a2:"walk_betw (to_dbltn ` insert e (t_set S)) (v2_of e) (v2_of e # q2) u"
-           using q_prop(1) 2(2)  by(intro walk_suff[of _ u "q1@[v1_of e]" "v2_of e" q2 u]) force 
-         ultimately have a3:"walk_betw (to_dbltn ` insert e (t_set S)) (v2_of e) ([v2_of e] @ q2) (v1_of e)"
-           by (simp add: "2"(3) walk_betw_def)
-         have a4:"set (edges_of_path ([v2_of e] @ q2)) \<subseteq> set (edges_of_path q)"
-           using "2"(2) "2"(3) by auto
-         moreover have a5:"to_dbltn e \<notin> set (edges_of_path ([v2_of e] @ q2))" 
-           using "2"(2) "2"(3) distinct_edges_q by auto
-         ultimately have a6:"set (edges_of_path ([v2_of e] @ q2)) \<subseteq> (to_dbltn `(t_set S))" 
-           using a3 graph_abs.path_ball_edges' graph_abs_with_e walk_between_nonempty_pathD(1) by fastforce
-         have "walk_betw (to_dbltn `(t_set S)) (v2_of e) ([v2_of e] @ q2) (v1_of e)"  
-           using walk_betw_strengthen[OF a3 _ a6] 2(4) by simp
-         hence "walk_betw (to_dbltn `(t_set S)) (v1_of e) (rev ([v2_of e] @ q2)) (v2_of e)" 
-           by (meson walk_symmetric)
-         thus ?case
-           using 2(1) by simp         
-       next
-         case (3 a list)
-         hence a1:"walk_betw (to_dbltn ` insert e (t_set S)) u (q1 @ [v1_of e]) (v1_of e)"
-           using q_prop(1) by (intro walk_pref[of _ u q1 "v1_of e" "v2_of e # q2" u]) force
-         moreover have a2:"walk_betw (to_dbltn ` insert e (t_set S)) (v2_of e) (v2_of e # q2) u"
-           using q_prop(1) 3(2)  by(intro walk_suff[of _ u "q1@[v1_of e]" "v2_of e" q2 u]) force 
-         ultimately have a3:"walk_betw (to_dbltn ` insert e (t_set S)) (v2_of e) (q1@ [v1_of e] ) (v1_of e)"
-           by (simp add: "3"(4) walk_betw_def)
-         have a4:"set (edges_of_path (q1@ [v1_of e])) \<subseteq> set (edges_of_path q)" 
-           using 3(2-) edges_of_path_append_subset_2 by fastforce
-         moreover have a5:"to_dbltn e \<notin> set (edges_of_path (q1@ [v1_of e]))" 
-           using  distinct_edges_q by(unfold 3(2) edges_of_path_symmetric_split) simp
-         ultimately have a6:"set (edges_of_path (q1@ [v1_of e])) \<subseteq> (to_dbltn `(t_set S))" 
-           using a3 graph_abs.path_ball_edges' graph_abs_with_e walk_between_nonempty_pathD(1) by fastforce
-         have "walk_betw (to_dbltn `(t_set S)) (v2_of e) (q1@ [v1_of e]) (v1_of e)"  
-           using walk_betw_strengthen[OF a3 _ a6] 3(3) by simp
-         hence "walk_betw (to_dbltn `(t_set S)) (v1_of e) (rev (q1@ [v1_of e])) (v2_of e)" 
-           by (meson walk_symmetric)
-         thus ?case
-           using 3(1) by simp 
-       next
-         case (4 a list aa lista)
-         hence a1:"walk_betw (to_dbltn ` insert e (t_set S)) u (q1 @ [v1_of e]) (v1_of e)"
-           using q_prop(1) by (intro walk_pref[of _ u q1 "v1_of e" "v2_of e # q2" u]) force
-         moreover have a2:"walk_betw (to_dbltn ` insert e (t_set S)) (v2_of e) (v2_of e # q2) u"
-           using q_prop(1) 4(2)  by(intro walk_suff[of _ u "q1@[v1_of e]" "v2_of e" q2 u]) force     
-         have a4:"set (edges_of_path (q1@ [v1_of e])) \<subseteq> set (edges_of_path q)" 
-           using 4(2-) edges_of_path_append_subset_2 by fastforce
-         moreover have a5:"to_dbltn e \<notin> set (edges_of_path (q1@ [v1_of e]))" 
-           using  distinct_edges_q by(unfold 4(2) edges_of_path_symmetric_split) simp
-         ultimately have a6:"set (edges_of_path (q1@ [v1_of e])) \<subseteq> (to_dbltn `(t_set S))" 
-           using graph_abs.path_ball_edges' graph_abs_with_e walk_between_nonempty_pathD(1) by fastforce
-         have a4:"set (edges_of_path ([v2_of e] @ q2)) \<subseteq> set (edges_of_path q)"
-           using "4"(2) edges_of_path_append_subset by fastforce
-         moreover have a5:"to_dbltn e \<notin> set (edges_of_path ([v2_of e] @ q2))" 
-           using  "4"(4) distinct_edges_q by(unfold 4(2) edges_of_path_symmetric_split) simp 
-         moreover have a3:"walk_betw (to_dbltn ` insert e (t_set S)) (v2_of e) ([v2_of e] @ q2) u"
-           using a2 a1 by simp 
-         ultimately have a7:"set (edges_of_path ([v2_of e] @ q2)) \<subseteq> (to_dbltn `(t_set S))"
-           using  a1 a2 graph_abs.path_ball_edges' graph_abs_with_e walk_between_nonempty_pathD(1) by fast 
-         have "walk_betw (to_dbltn `(t_set S)) u (q1@ [v1_of e]) (v1_of e)"  
-           using walk_betw_strengthen 4(3) a1 a6 by fastforce
-         moreover have "walk_betw (to_dbltn `(t_set S)) (v2_of e) ( [v2_of e]@q2)u"  
-           using walk_betw_strengthen 4(3)  "4"(4) a3 a7 by fastforce
-         ultimately have  "walk_betw (to_dbltn `(t_set S)) (v2_of e) ( ([v2_of e]@q2@(tl q1)@[v1_of e])) (v1_of e)" 
-           using "4"(3) walk_transitive_2 by fastforce
-         then show ?case 
-           using 4(1)[of "rev ([v2_of e]@q2@(tl q1)@[v1_of e])"]
-           by (meson walk_symmetric)
-       next
-         case 5
-         then show ?case 
-           using q_prop(1) v1v2 walk_between_nonempty_pathD(3) walk_between_nonempty_pathD(4) by fastforce
-       next
-         case (6 a list)
-         hence a1:"walk_betw (to_dbltn ` insert e (t_set S)) u (q1 @ [v2_of e]) (v2_of e)"
-           using q_prop(1) by (intro walk_pref[of _ u q1 "v2_of e" "v1_of e # q2" u]) force
-         moreover have a2:"walk_betw (to_dbltn ` insert e (t_set S)) (v1_of e) (v1_of e # q2) u"
-           using q_prop(1) 6(2)  by(intro walk_suff[of _ u "q1@[v2_of e]" "v1_of e" q2 u]) force 
-         ultimately have a3:"walk_betw (to_dbltn ` insert e (t_set S)) (v1_of e) ([v1_of e] @ q2) (v2_of e)"
-           by (simp add: "6"(3) walk_betw_def)
-         have a4:"set (edges_of_path ([v1_of e] @ q2)) \<subseteq> set (edges_of_path q)"
-           using "6"(2) "6"(3) by auto
-         moreover have a5:"to_dbltn e \<notin> set (edges_of_path ([v1_of e] @ q2))" 
-           using "6"(2) "6"(3) distinct_edges_q 
-           by (simp add: insert_commute)
-         ultimately have a6:"set (edges_of_path ([v1_of e] @ q2)) \<subseteq> (to_dbltn `(t_set S))" 
-           using a3 graph_abs.path_ball_edges' graph_abs_with_e walk_between_nonempty_pathD(1) by fastforce
-         have "walk_betw (to_dbltn `(t_set S)) (v1_of e) ([v1_of e] @ q2) (v2_of e)"  
-           using walk_betw_strengthen[OF a3 _ a6] 6(4) by simp
-         thus ?case
-           using 6(1) by simp         
-       next
-         case (7 a list)
-         hence a1:"walk_betw (to_dbltn ` insert e (t_set S)) u (q1 @ [v2_of e]) (v2_of e)"
-           using q_prop(1) by (intro walk_pref[of _ u q1 "v2_of e" "v1_of e # q2" u]) force
-         moreover have a2:"walk_betw (to_dbltn ` insert e (t_set S)) (v1_of e) (v1_of e # q2) u"
-           using q_prop(1) 7(2)  by(intro walk_suff[of _ u "q1@[v2_of e]" "v1_of e" q2 u]) force 
-         ultimately have a3:"walk_betw (to_dbltn ` insert e (t_set S)) (v1_of e) (q1@ [v2_of e] ) (v2_of e)"
-           by (simp add: "7"(4) walk_betw_def)
-         have a4:"set (edges_of_path (q1@ [v2_of e])) \<subseteq> set (edges_of_path q)" 
-           using 7(2-) edges_of_path_append_subset_2 by fastforce
-         moreover have a5:"to_dbltn e \<notin> set (edges_of_path (q1@ [v2_of e]))" 
-           using  distinct_edges_q by(unfold 7(2) edges_of_path_symmetric_split to_dbltn_sym) auto
-         ultimately have a6:"set (edges_of_path (q1@ [v2_of e])) \<subseteq> (to_dbltn `(t_set S))" 
-           using a3 graph_abs.path_ball_edges' graph_abs_with_e walk_between_nonempty_pathD(1) by fastforce
-         have "walk_betw (to_dbltn `(t_set S)) (v1_of e) (q1@ [v2_of e]) (v2_of e)"  
-           using walk_betw_strengthen[OF a3 _ a6] 7(3) by simp
-         thus ?case
-           using 7(1) by simp 
-       next
-         case (8 a list aa lista)
-         hence a1:"walk_betw (to_dbltn ` insert e (t_set S)) u (q1 @ [v2_of e]) (v2_of e)"
-           using q_prop(1) by (intro walk_pref[of _ u q1 "v2_of e" "v1_of e # q2" u]) force
-         moreover have a2:"walk_betw (to_dbltn ` insert e (t_set S)) (v1_of e) (v1_of e # q2) u"
-           using q_prop(1) 8(2)  by(intro walk_suff[of _ u "q1@[v2_of e]" "v1_of e" q2 u]) force     
-         have a4:"set (edges_of_path (q1@ [v2_of e])) \<subseteq> set (edges_of_path q)" 
-           using 8(2-) edges_of_path_append_subset_2 by fastforce
-         moreover have a5:"to_dbltn e \<notin> set (edges_of_path (q1@ [v2_of e]))" 
-           using  distinct_edges_q by(unfold 8(2) edges_of_path_symmetric_split to_dbltn_sym) simp
-         ultimately have a6:"set (edges_of_path (q1@ [v2_of e])) \<subseteq> (to_dbltn `(t_set S))" 
-           using graph_abs.path_ball_edges' graph_abs_with_e walk_between_nonempty_pathD(1) by fastforce
-         have a4:"set (edges_of_path ([v1_of e] @ q2)) \<subseteq> set (edges_of_path q)"
-           using 8(2) edges_of_path_append_subset by fastforce
-         moreover have a5:"to_dbltn e \<notin> set (edges_of_path ([v1_of e] @ q2))" 
-           using 8(4) distinct_edges_q by(unfold 8(2) edges_of_path_symmetric_split to_dbltn_sym) simp 
-         moreover have a3:"walk_betw (to_dbltn ` insert e (t_set S)) (v1_of e) ([v1_of e] @ q2) u"
-           using a2 a1 by simp 
-         ultimately have a7:"set (edges_of_path ([v1_of e] @ q2)) \<subseteq> (to_dbltn `(t_set S))"
-           using  a1 a2 graph_abs.path_ball_edges' graph_abs_with_e walk_between_nonempty_pathD(1) by fast 
-         have "walk_betw (to_dbltn `(t_set S)) u (q1@ [v2_of e]) (v2_of e)"  
-           using walk_betw_strengthen 8(3) a1 a6 by fastforce
-         moreover have "walk_betw (to_dbltn `(t_set S)) (v1_of e) ( [v1_of e]@q2)u"  
-           using walk_betw_strengthen 8(3)  8(4) a3 a7 by fastforce
-         ultimately have  "walk_betw (to_dbltn `(t_set S)) (v1_of e) ( ([v1_of e]@q2@(tl q1)@[v2_of e])) (v2_of e)" 
-           using 8(3) walk_transitive_2 by fastforce
-         then show ?case using 8(1) by auto
-       qed
-       have  dfs_vwalk:"vwalk_bet (dfs.Graph.digraph_abs (local.Kruskal_E_to_G S)) (v1_of e) q' (v2_of e)"
-         apply(subst same_dgraphabs, subst Pair_Graph_U_RBT.ugraph_abs_digraph_abs[symmetric])
-         using local.Kruskal_E_to_G_def pair_graph_u_invar apply simp
-         using  graph_abs.walk_betw_iff_vwalk_bet[OF graph_abs_without_e]  path_without_e 
-         by (simp  add: ugraph_abs_is )
-       obtain q'' where "vwalk_bet (dfs.Graph.digraph_abs (local.Kruskal_E_to_G S)) (v1_of e) q'' (v2_of e)"
-                             "distinct q''" 
-         using  vwalk_bet_to_distinct_is_distinct_vwalk_bet[OF dfs_vwalk]
-         by(auto simp add: distinct_vwalk_bet_def)
-       thus False 
-         using no_distinct_path by blast
-     qed
-   next
-     case 2
-     note two = this
-     show ?case 
-     proof(cases "lookup (local.Kruskal_E_to_G S) (v2_of e)")
-       case None 
-       hence "lookup (local.Kruskal_E_to_G S) (v1_of e) = None" 
-         using two(2) by blast
-       thus False 
-         by (simp add: one)
-     next
-       case (Some neighbs)
-       hence dfs_reachable:"return
+              by fastforce
+            moreover have "distinct [v1_of e, v2_of e]"
+              using v1v2 by auto
+            ultimately show ?case 
+              using   no_distinct_path by blast
+          qed 
+          moreover have dbltn_inj:"inj_on to_dbltn (t_set S) "
+            using case_assms(2) undirected_multigraph.has_no_cycle_multi_to_dbltn_inj by simp
+          ultimately have dbltn_inj_big:"inj_on to_dbltn (insert e (t_set S))" by auto
+          moreover have C_subset:"set C \<subseteq> (insert e (t_set S))"
+            using case_assms(1) dfs.Graph.vset.set.set_insert e_and_C(2) by auto
+          ultimately have inj_C:"inj_on to_dbltn (set C)" 
+            by (meson inj_on_subset)
+          have distinct_edges_q:"distinct (edges_of_path q)"
+            using q_prop(2) distinct_map[of to_dbltn C] uC_prop e_and_C inj_C
+            by(auto simp add: undirected_multigraph.decycle_multi_def) 
+          have e_vs_in_new_v_set:"{v1_of e, v2_of e} \<subseteq> Vs (to_dbltn ` insert e (t_set S))"
+            by (simp add: vs_member)
+          then obtain q1 q2 where q1_q2_prop: "q = q1@[v1_of e, v2_of e]@ q2 \<or> q = q1@[v2_of e, v1_of e]@ q2"
+            using undirected_multigraph.edges_to_path_split_by_edge[of _ _ "v1_of e" "v2_of e"] e_in_p by fast
+          obtain q' where  path_without_e:"walk_betw (to_dbltn `  (t_set S)) (v1_of e) q' (v2_of e)"
+          proof(cases rule: disjE[OF q1_q2_prop], all "cases q1", all \<open>cases q2\<close>, goal_cases)
+            case 1
+            then show ?case 
+              using q_prop(1) v1v2 walk_between_nonempty_pathD(3) walk_between_nonempty_pathD(4) by fastforce
+          next
+            case (2 a list)
+            hence a1:"walk_betw (to_dbltn ` insert e (t_set S)) u (q1 @ [v1_of e]) (v1_of e)"
+              using q_prop(1) by (intro walk_pref[of _ u q1 "v1_of e" "v2_of e # q2" u]) force
+            moreover have a2:"walk_betw (to_dbltn ` insert e (t_set S)) (v2_of e) (v2_of e # q2) u"
+              using q_prop(1) 2(2)  by(intro walk_suff[of _ u "q1@[v1_of e]" "v2_of e" q2 u]) force 
+            ultimately have a3:"walk_betw (to_dbltn ` insert e (t_set S)) (v2_of e) ([v2_of e] @ q2) (v1_of e)"
+              by (simp add: "2"(3) walk_betw_def)
+            have a4:"set (edges_of_path ([v2_of e] @ q2)) \<subseteq> set (edges_of_path q)"
+              using "2"(2) "2"(3) by auto
+            moreover have a5:"to_dbltn e \<notin> set (edges_of_path ([v2_of e] @ q2))" 
+              using "2"(2) "2"(3) distinct_edges_q by auto
+            ultimately have a6:"set (edges_of_path ([v2_of e] @ q2)) \<subseteq> (to_dbltn `(t_set S))" 
+              using a3 graph_abs.path_ball_edges' graph_abs_with_e walk_between_nonempty_pathD(1) by fastforce
+            have "walk_betw (to_dbltn `(t_set S)) (v2_of e) ([v2_of e] @ q2) (v1_of e)"  
+              using walk_betw_strengthen[OF a3 _ a6] 2(4) by simp
+            hence "walk_betw (to_dbltn `(t_set S)) (v1_of e) (rev ([v2_of e] @ q2)) (v2_of e)" 
+              by (meson walk_symmetric)
+            thus ?case
+              using 2(1) by simp         
+          next
+            case (3 a list)
+            hence a1:"walk_betw (to_dbltn ` insert e (t_set S)) u (q1 @ [v1_of e]) (v1_of e)"
+              using q_prop(1) by (intro walk_pref[of _ u q1 "v1_of e" "v2_of e # q2" u]) force
+            moreover have a2:"walk_betw (to_dbltn ` insert e (t_set S)) (v2_of e) (v2_of e # q2) u"
+              using q_prop(1) 3(2)  by(intro walk_suff[of _ u "q1@[v1_of e]" "v2_of e" q2 u]) force 
+            ultimately have a3:"walk_betw (to_dbltn ` insert e (t_set S)) (v2_of e) (q1@ [v1_of e] ) (v1_of e)"
+              by (simp add: "3"(4) walk_betw_def)
+            have a4:"set (edges_of_path (q1@ [v1_of e])) \<subseteq> set (edges_of_path q)" 
+              using 3(2-) edges_of_path_append_subset_2 by fastforce
+            moreover have a5:"to_dbltn e \<notin> set (edges_of_path (q1@ [v1_of e]))" 
+              using  distinct_edges_q by(unfold 3(2) edges_of_path_symmetric_split) simp
+            ultimately have a6:"set (edges_of_path (q1@ [v1_of e])) \<subseteq> (to_dbltn `(t_set S))" 
+              using a3 graph_abs.path_ball_edges' graph_abs_with_e walk_between_nonempty_pathD(1) by fastforce
+            have "walk_betw (to_dbltn `(t_set S)) (v2_of e) (q1@ [v1_of e]) (v1_of e)"  
+              using walk_betw_strengthen[OF a3 _ a6] 3(3) by simp
+            hence "walk_betw (to_dbltn `(t_set S)) (v1_of e) (rev (q1@ [v1_of e])) (v2_of e)" 
+              by (meson walk_symmetric)
+            thus ?case
+              using 3(1) by simp 
+          next
+            case (4 a list aa lista)
+            hence a1:"walk_betw (to_dbltn ` insert e (t_set S)) u (q1 @ [v1_of e]) (v1_of e)"
+              using q_prop(1) by (intro walk_pref[of _ u q1 "v1_of e" "v2_of e # q2" u]) force
+            moreover have a2:"walk_betw (to_dbltn ` insert e (t_set S)) (v2_of e) (v2_of e # q2) u"
+              using q_prop(1) 4(2)  by(intro walk_suff[of _ u "q1@[v1_of e]" "v2_of e" q2 u]) force     
+            have a4:"set (edges_of_path (q1@ [v1_of e])) \<subseteq> set (edges_of_path q)" 
+              using 4(2-) edges_of_path_append_subset_2 by fastforce
+            moreover have a5:"to_dbltn e \<notin> set (edges_of_path (q1@ [v1_of e]))" 
+              using  distinct_edges_q by(unfold 4(2) edges_of_path_symmetric_split) simp
+            ultimately have a6:"set (edges_of_path (q1@ [v1_of e])) \<subseteq> (to_dbltn `(t_set S))" 
+              using graph_abs.path_ball_edges' graph_abs_with_e walk_between_nonempty_pathD(1) by fastforce
+            have a4:"set (edges_of_path ([v2_of e] @ q2)) \<subseteq> set (edges_of_path q)"
+              using "4"(2) edges_of_path_append_subset by fastforce
+            moreover have a5:"to_dbltn e \<notin> set (edges_of_path ([v2_of e] @ q2))" 
+              using  "4"(4) distinct_edges_q by(unfold 4(2) edges_of_path_symmetric_split) simp 
+            moreover have a3:"walk_betw (to_dbltn ` insert e (t_set S)) (v2_of e) ([v2_of e] @ q2) u"
+              using a2 a1 by simp 
+            ultimately have a7:"set (edges_of_path ([v2_of e] @ q2)) \<subseteq> (to_dbltn `(t_set S))"
+              using  a1 a2 graph_abs.path_ball_edges' graph_abs_with_e walk_between_nonempty_pathD(1) by fast 
+            have "walk_betw (to_dbltn `(t_set S)) u (q1@ [v1_of e]) (v1_of e)"  
+              using walk_betw_strengthen 4(3) a1 a6 by fastforce
+            moreover have "walk_betw (to_dbltn `(t_set S)) (v2_of e) ( [v2_of e]@q2)u"  
+              using walk_betw_strengthen 4(3)  "4"(4) a3 a7 by fastforce
+            ultimately have  "walk_betw (to_dbltn `(t_set S)) (v2_of e) ( ([v2_of e]@q2@(tl q1)@[v1_of e])) (v1_of e)" 
+              using "4"(3) walk_transitive_2 by fastforce
+            then show ?case 
+              using 4(1)[of "rev ([v2_of e]@q2@(tl q1)@[v1_of e])"]
+              by (meson walk_symmetric)
+          next
+            case 5
+            then show ?case 
+              using q_prop(1) v1v2 walk_between_nonempty_pathD(3) walk_between_nonempty_pathD(4) by fastforce
+          next
+            case (6 a list)
+            hence a1:"walk_betw (to_dbltn ` insert e (t_set S)) u (q1 @ [v2_of e]) (v2_of e)"
+              using q_prop(1) by (intro walk_pref[of _ u q1 "v2_of e" "v1_of e # q2" u]) force
+            moreover have a2:"walk_betw (to_dbltn ` insert e (t_set S)) (v1_of e) (v1_of e # q2) u"
+              using q_prop(1) 6(2)  by(intro walk_suff[of _ u "q1@[v2_of e]" "v1_of e" q2 u]) force 
+            ultimately have a3:"walk_betw (to_dbltn ` insert e (t_set S)) (v1_of e) ([v1_of e] @ q2) (v2_of e)"
+              by (simp add: "6"(3) walk_betw_def)
+            have a4:"set (edges_of_path ([v1_of e] @ q2)) \<subseteq> set (edges_of_path q)"
+              using "6"(2) "6"(3) by auto
+            moreover have a5:"to_dbltn e \<notin> set (edges_of_path ([v1_of e] @ q2))" 
+              using "6"(2) "6"(3) distinct_edges_q 
+              by (simp add: insert_commute)
+            ultimately have a6:"set (edges_of_path ([v1_of e] @ q2)) \<subseteq> (to_dbltn `(t_set S))" 
+              using a3 graph_abs.path_ball_edges' graph_abs_with_e walk_between_nonempty_pathD(1) by fastforce
+            have "walk_betw (to_dbltn `(t_set S)) (v1_of e) ([v1_of e] @ q2) (v2_of e)"  
+              using walk_betw_strengthen[OF a3 _ a6] 6(4) by simp
+            thus ?case
+              using 6(1) by simp         
+          next
+            case (7 a list)
+            hence a1:"walk_betw (to_dbltn ` insert e (t_set S)) u (q1 @ [v2_of e]) (v2_of e)"
+              using q_prop(1) by (intro walk_pref[of _ u q1 "v2_of e" "v1_of e # q2" u]) force
+            moreover have a2:"walk_betw (to_dbltn ` insert e (t_set S)) (v1_of e) (v1_of e # q2) u"
+              using q_prop(1) 7(2)  by(intro walk_suff[of _ u "q1@[v2_of e]" "v1_of e" q2 u]) force 
+            ultimately have a3:"walk_betw (to_dbltn ` insert e (t_set S)) (v1_of e) (q1@ [v2_of e] ) (v2_of e)"
+              by (simp add: "7"(4) walk_betw_def)
+            have a4:"set (edges_of_path (q1@ [v2_of e])) \<subseteq> set (edges_of_path q)" 
+              using 7(2-) edges_of_path_append_subset_2 by fastforce
+            moreover have a5:"to_dbltn e \<notin> set (edges_of_path (q1@ [v2_of e]))" 
+              using  distinct_edges_q by(unfold 7(2) edges_of_path_symmetric_split to_dbltn_sym) auto
+            ultimately have a6:"set (edges_of_path (q1@ [v2_of e])) \<subseteq> (to_dbltn `(t_set S))" 
+              using a3 graph_abs.path_ball_edges' graph_abs_with_e walk_between_nonempty_pathD(1) by fastforce
+            have "walk_betw (to_dbltn `(t_set S)) (v1_of e) (q1@ [v2_of e]) (v2_of e)"  
+              using walk_betw_strengthen[OF a3 _ a6] 7(3) by simp
+            thus ?case
+              using 7(1) by simp 
+          next
+            case (8 a list aa lista)
+            hence a1:"walk_betw (to_dbltn ` insert e (t_set S)) u (q1 @ [v2_of e]) (v2_of e)"
+              using q_prop(1) by (intro walk_pref[of _ u q1 "v2_of e" "v1_of e # q2" u]) force
+            moreover have a2:"walk_betw (to_dbltn ` insert e (t_set S)) (v1_of e) (v1_of e # q2) u"
+              using q_prop(1) 8(2)  by(intro walk_suff[of _ u "q1@[v2_of e]" "v1_of e" q2 u]) force     
+            have a4:"set (edges_of_path (q1@ [v2_of e])) \<subseteq> set (edges_of_path q)" 
+              using 8(2-) edges_of_path_append_subset_2 by fastforce
+            moreover have a5:"to_dbltn e \<notin> set (edges_of_path (q1@ [v2_of e]))" 
+              using  distinct_edges_q by(unfold 8(2) edges_of_path_symmetric_split to_dbltn_sym) simp
+            ultimately have a6:"set (edges_of_path (q1@ [v2_of e])) \<subseteq> (to_dbltn `(t_set S))" 
+              using graph_abs.path_ball_edges' graph_abs_with_e walk_between_nonempty_pathD(1) by fastforce
+            have a4:"set (edges_of_path ([v1_of e] @ q2)) \<subseteq> set (edges_of_path q)"
+              using 8(2) edges_of_path_append_subset by fastforce
+            moreover have a5:"to_dbltn e \<notin> set (edges_of_path ([v1_of e] @ q2))" 
+              using 8(4) distinct_edges_q by(unfold 8(2) edges_of_path_symmetric_split to_dbltn_sym) simp 
+            moreover have a3:"walk_betw (to_dbltn ` insert e (t_set S)) (v1_of e) ([v1_of e] @ q2) u"
+              using a2 a1 by simp 
+            ultimately have a7:"set (edges_of_path ([v1_of e] @ q2)) \<subseteq> (to_dbltn `(t_set S))"
+              using  a1 a2 graph_abs.path_ball_edges' graph_abs_with_e walk_between_nonempty_pathD(1) by fast 
+            have "walk_betw (to_dbltn `(t_set S)) u (q1@ [v2_of e]) (v2_of e)"  
+              using walk_betw_strengthen 8(3) a1 a6 by fastforce
+            moreover have "walk_betw (to_dbltn `(t_set S)) (v1_of e) ( [v1_of e]@q2)u"  
+              using walk_betw_strengthen 8(3)  8(4) a3 a7 by fastforce
+            ultimately have  "walk_betw (to_dbltn `(t_set S)) (v1_of e) ( ([v1_of e]@q2@(tl q1)@[v2_of e])) (v2_of e)" 
+              using 8(3) walk_transitive_2 by fastforce
+            then show ?case using 8(1) by auto
+          qed
+          have  dfs_vwalk:"vwalk_bet (dfs.Graph.digraph_abs (local.Kruskal_E_to_G S)) (v1_of e) q' (v2_of e)"
+            apply(subst same_dgraphabs, subst Pair_Graph_U_RBT.ugraph_abs_digraph_abs[symmetric])
+            using local.Kruskal_E_to_G_def pair_graph_u_invar apply simp
+            using  graph_abs.walk_betw_iff_vwalk_bet[OF graph_abs_without_e]  path_without_e 
+            by (simp  add: ugraph_abs_is )
+          obtain q'' where "vwalk_bet (dfs.Graph.digraph_abs (local.Kruskal_E_to_G S)) (v1_of e) q'' (v2_of e)"
+            "distinct q''" 
+            using  vwalk_bet_to_distinct_is_distinct_vwalk_bet[OF dfs_vwalk]
+            by(auto simp add: distinct_vwalk_bet_def)
+          thus False 
+            using no_distinct_path by blast
+        qed
+      next
+        case 2
+        note two = this
+        show ?case 
+        proof(cases "lookup (local.Kruskal_E_to_G S) (v2_of e)")
+          case None 
+          hence "lookup (local.Kruskal_E_to_G S) (v1_of e) = None" 
+            using two(2) by blast
+          thus False 
+            by (simp add: one)
+        next
+          case (Some neighbs)
+          hence dfs_reachable:"return
          (dfs.DFS (local.Kruskal_E_to_G S) (v2_of e) (DFS.initial_state vset_insert vset_empty (v1_of e))) =
              Reachable" 
-         using two(2) return.exhaust by auto
-       then obtain p where p_vwalk:"vwalk_bet (dfs.Graph.digraph_abs (local.Kruskal_E_to_G S)) (v1_of e)
+            using two(2) return.exhaust by auto
+          then obtain p where p_vwalk:"vwalk_bet (dfs.Graph.digraph_abs (local.Kruskal_E_to_G S)) (v1_of e)
                                       p (v2_of e)"
-         using DFS_thms.DFS_correct_2[OF DFS_thms[OF one(1)]] dfs_reachable by auto
-       have walk_betw_around_e:"walk_betw (to_dbltn ` t_set S) (v1_of e) p (v2_of e)"
-         apply(subst  ugraph_abs_is[symmetric], subst graph_abs.walk_betw_iff_vwalk_bet, simp add: graph_abs_without_e ugraph_abs_is)
-         using  pair_graph_u_invar  p_vwalk 
-         by(auto simp add: Pair_Graph_U_RBT.ugraph_abs_digraph_abs same_dgraphabs Kruskal_E_to_G_def)
-       have "epath (to_dbltn ` t_set S) (v1_of e) (edges_of_path p) (v2_of e)" 
-         by(auto intro!: graph_abs.walk_betw_imp_epath simp add: walk_betw_around_e graph_abs_without_e)
-       moreover then obtain p' where p'_prop:"map to_dbltn p' = edges_of_path p" "set p' \<subseteq>  (t_set S)"
-         using undirected_multigraph.edges_of_path_to_multigraph_path[OF epath_edges_subset]
-         by blast 
-       ultimately have epath_first_path:"epath (to_dbltn `  (t_set S)) (v1_of e) (map to_dbltn p') (v2_of e)"  
-         by simp
-       then obtain p'' where p''_prop:"epath (to_dbltn ` t_set S) (v1_of e) p'' (v2_of e)" 
-                       "set p'' \<subseteq> set (map to_dbltn p')" "distinct p''"
-         using  epath_distinct_epath by fast
-       obtain p_mul where p_mul: "map to_dbltn p_mul = p''" "set p_mul \<subseteq> set p'"
-         using p''_prop(2) map_eq_Cons_conv by(induction p'')  fastforce+
-       hence epath_p_mul:"epath (to_dbltn ` t_set S) (v1_of e) (map to_dbltn p_mul) (v2_of e)"
-         using p''_prop(1) by blast
-       hence epath_first_path:"epath (to_dbltn ` (insert e (t_set S))) (v1_of e) (map to_dbltn p_mul) (v2_of e)"  
-         by (auto intro: epath_subset image_mono subset_insertI)
-       moreover have "epath (to_dbltn ` (insert e (t_set S))) (v2_of e) [to_dbltn e] (v1_of e)" 
-         using v1_never_v2[of e] by(auto intro!: epath_single)
-       ultimately have epath3:"epath (to_dbltn ` (insert e (t_set S))) (v1_of e) 
+            using DFS_thms.DFS_correct_2[OF DFS_thms[OF one(1)]] dfs_reachable by auto
+          have walk_betw_around_e:"walk_betw (to_dbltn ` t_set S) (v1_of e) p (v2_of e)"
+            apply(subst  ugraph_abs_is[symmetric], subst graph_abs.walk_betw_iff_vwalk_bet, simp add: graph_abs_without_e ugraph_abs_is)
+            using  pair_graph_u_invar  p_vwalk 
+            by(auto simp add: Pair_Graph_U_RBT.ugraph_abs_digraph_abs same_dgraphabs Kruskal_E_to_G_def)
+          have "epath (to_dbltn ` t_set S) (v1_of e) (edges_of_path p) (v2_of e)" 
+            by(auto intro!: graph_abs.walk_betw_imp_epath simp add: walk_betw_around_e graph_abs_without_e)
+          moreover then obtain p' where p'_prop:"map to_dbltn p' = edges_of_path p" "set p' \<subseteq>  (t_set S)"
+            using undirected_multigraph.edges_of_path_to_multigraph_path[OF epath_edges_subset]
+            by blast 
+          ultimately have epath_first_path:"epath (to_dbltn `  (t_set S)) (v1_of e) (map to_dbltn p') (v2_of e)"  
+            by simp
+          then obtain p'' where p''_prop:"epath (to_dbltn ` t_set S) (v1_of e) p'' (v2_of e)" 
+            "set p'' \<subseteq> set (map to_dbltn p')" "distinct p''"
+            using  epath_distinct_epath by fast
+          obtain p_mul where p_mul: "map to_dbltn p_mul = p''" "set p_mul \<subseteq> set p'"
+            using p''_prop(2) map_eq_Cons_conv by(induction p'')  fastforce+
+          hence epath_p_mul:"epath (to_dbltn ` t_set S) (v1_of e) (map to_dbltn p_mul) (v2_of e)"
+            using p''_prop(1) by blast
+          hence epath_first_path:"epath (to_dbltn ` (insert e (t_set S))) (v1_of e) (map to_dbltn p_mul) (v2_of e)"  
+            by (auto intro: epath_subset image_mono subset_insertI)
+          moreover have "epath (to_dbltn ` (insert e (t_set S))) (v2_of e) [to_dbltn e] (v1_of e)" 
+            using v1_never_v2[of e] by(auto intro!: epath_single)
+          ultimately have epath3:"epath (to_dbltn ` (insert e (t_set S))) (v1_of e) 
                               (map to_dbltn (p_mul@[e])) (v1_of e)" 
-         by (auto intro: epath_append)
-       moreover have "set (p_mul@[e]) \<subseteq> insert e (t_set S)" 
-         using p'_prop(2) p_mul(2) by auto
-       moreover have "2 \<le> length (p_mul@[e])" 
-         using epath_non_empty[OF epath_p_mul, simplified length_map] 
-         by (simp add: v1_never_v2)
-       moreover have "distinct (p_mul@[e])" 
-       proof-
-         have "distinct p_mul"
-           using p_mul(1)  p''_prop(3) by (auto simp add: distinct_map)
-         moreover have "set p_mul \<subseteq> t_set S" 
-           using p'_prop(2) p_mul(2) by order
-         ultimately show ?thesis using assms(4) by auto
-       qed
-       ultimately have "undirected_multigraph.decycle_multi (t_set (vset_insert e (id S))) (v1_of e) (p_mul@[e])" 
-          by (simp add: undirected_multigraph.decycle_multi_def  case_assms(1) dfs.Graph.vset.set.set_insert)
-        thus ?thesis 
-         using 2(1) by simp
-     qed
-   qed
- next
-   case 2
-   have "(\<nexists>u. Ex (undirected_multigraph.decycle_multi (t_set (vset_insert e (id S))) u))"
-   proof(rule ccontr,goal_cases)
-     case 1
-     then obtain u C where uC:"undirected_multigraph.decycle_multi (insert e (t_set S)) u C"
-       using case_assms(1) dfs.Graph.vset.set.set_insert by fastforce
-     hence C_prop: "epath (to_dbltn ` insert e (t_set S)) u (map to_dbltn C) u"
-                    "set C \<subseteq> insert e (t_set S)" " 2 \<le> length C" "distinct C"
-       using uC[simplified undirected_multigraph.decycle_multi_def] by auto
-     have e_in_C:"e \<in> set C"
-     proof(rule ccontr, goal_cases)
-       case 1
-       hence "undirected_multigraph.decycle_multi (t_set S) u C"
-         using uC epath_subset_other_set[of "(to_dbltn ` insert e (t_set S))" 
-                    u "map to_dbltn C" u "to_dbltn ` (t_set S)"] 
-         by (simp add: image_mono subset_insert undirected_multigraph.decycle_multi_def)
-       then show ?case 
-         using assms(2)  case_assms(2) by(force simp add: undirected_multigraph.has_no_cycle_multi_def)
-     qed
-     obtain C1 C2 where C1C2:"C = C1@[e]@C2"
-       by (metis append_Cons append_Nil e_in_C in_set_conv_decomp_first)
-     hence epath_extended:"epath  (to_dbltn ` insert e (t_set S)) u (map to_dbltn (C1@[e]@C2@C1@[e]@C2@C1@[e]@C2)) u"
-       using epath_append C_prop(1)[simplified C1C2] by fastforce
-     have middle_three_rewrite:"xs@[x,y,z]@ys = (xs@[x])@[y]@(z#ys)" for x y z xs ys by auto
-     have e_path_very_verbose: "epath (to_dbltn ` insert e (t_set S)) u
+            by (auto intro: epath_append)
+          moreover have "set (p_mul@[e]) \<subseteq> insert e (t_set S)" 
+            using p'_prop(2) p_mul(2) by auto
+          moreover have "2 \<le> length (p_mul@[e])" 
+            using epath_non_empty[OF epath_p_mul, simplified length_map] 
+            by (simp add: v1_never_v2)
+          moreover have "distinct (p_mul@[e])" 
+          proof-
+            have "distinct p_mul"
+              using p_mul(1)  p''_prop(3) by (auto simp add: distinct_map)
+            moreover have "set p_mul \<subseteq> t_set S" 
+              using p'_prop(2) p_mul(2) by order
+            ultimately show ?thesis using assms(4) by auto
+          qed
+          ultimately have "undirected_multigraph.decycle_multi (t_set (vset_insert e (id S))) (v1_of e) (p_mul@[e])" 
+            by (simp add: undirected_multigraph.decycle_multi_def  case_assms(1) dfs.Graph.vset.set.set_insert)
+          thus ?thesis 
+            using 2(1) by simp
+        qed
+      qed
+    next
+      case 2
+      have "(\<nexists>u. Ex (undirected_multigraph.decycle_multi (t_set (vset_insert e (id S))) u))"
+      proof(rule ccontr,goal_cases)
+        case 1
+        then obtain u C where uC:"undirected_multigraph.decycle_multi (insert e (t_set S)) u C"
+          using case_assms(1) dfs.Graph.vset.set.set_insert by fastforce
+        hence C_prop: "epath (to_dbltn ` insert e (t_set S)) u (map to_dbltn C) u"
+          "set C \<subseteq> insert e (t_set S)" " 2 \<le> length C" "distinct C"
+          using uC[simplified undirected_multigraph.decycle_multi_def] by auto
+        have e_in_C:"e \<in> set C"
+        proof(rule ccontr, goal_cases)
+          case 1
+          hence "undirected_multigraph.decycle_multi (t_set S) u C"
+            using uC epath_subset_other_set[of "(to_dbltn ` insert e (t_set S))" 
+                u "map to_dbltn C" u "to_dbltn ` (t_set S)"] 
+            by (simp add: image_mono subset_insert undirected_multigraph.decycle_multi_def)
+          then show ?case 
+            using assms(2)  case_assms(2) by(force simp add: undirected_multigraph.has_no_cycle_multi_def)
+        qed
+        obtain C1 C2 where C1C2:"C = C1@[e]@C2"
+          by (metis append_Cons append_Nil e_in_C in_set_conv_decomp_first)
+        hence epath_extended:"epath  (to_dbltn ` insert e (t_set S)) u (map to_dbltn (C1@[e]@C2@C1@[e]@C2@C1@[e]@C2)) u"
+          using epath_append C_prop(1)[simplified C1C2] by fastforce
+        have middle_three_rewrite:"xs@[x,y,z]@ys = (xs@[x])@[y]@(z#ys)" for x y z xs ys by auto
+        have e_path_very_verbose: "epath (to_dbltn ` insert e (t_set S)) u
  (butlast (map to_dbltn (C1 @ [e] @ C2 @ C1)) @
   [last (map to_dbltn (C1 @ [e] @ C2 @ C1)), to_dbltn e, hd (map to_dbltn (C2 @ C1 @ [e] @ C2))] @
   tl (map to_dbltn (C2 @ C1 @ [e] @ C2))) u"
-       using epath_extended
-       apply(rule back_subst[of "\<lambda> p. epath _ _ p _ "])
-       apply(subst middle_three_rewrite) 
-       apply(subst append_butlast_last_id, simp)
-       apply(subst hd_Cons_tl,simp)
-       by auto
-     have "\<exists>x y. to_dbltn e = {x, y} \<and>
+          using epath_extended
+          apply(rule back_subst[of "\<lambda> p. epath _ _ p _ "])
+          apply(subst middle_three_rewrite) 
+          apply(subst append_butlast_last_id, simp)
+          apply(subst hd_Cons_tl,simp)
+          by auto
+        have "\<exists>x y. to_dbltn e = {x, y} \<and>
       x \<noteq> y \<and>
       epath (to_dbltn ` insert e (t_set S)) u
        (butlast (map to_dbltn (C1 @ [e] @ C2 @ C1)) @ [last (map to_dbltn (C1 @ [e] @ C2 @ C1))]) x \<and>
@@ -743,115 +725,115 @@ proof(goal_cases)
        ([hd (map to_dbltn (C2 @ C1 @ [e] @ C2))] @ tl (map to_dbltn (C2 @ C1 @ [e] @ C2))) u \<and>
       x \<in> last (map to_dbltn (C1 @ [e] @ C2 @ C1)) \<inter> to_dbltn e \<and>
       y \<in> to_dbltn e \<inter> hd (map to_dbltn (C2 @ C1 @ [e] @ C2))"
-       using epath_find_splitter_advanced[OF e_path_very_verbose] by simp
-     then obtain x y where xy_prop:"to_dbltn e = {x, y}"
-      "x \<noteq> y"
-      "epath (to_dbltn ` insert e (t_set S)) u (map to_dbltn (C1 @ [e] @ C2 @ C1)) x"
-      "epath (to_dbltn ` insert e (t_set S)) y (map to_dbltn (C2 @ C1 @ [e] @ C2)) u"
-      "x \<in> last (map to_dbltn (C1 @ [e] @ C2 @ C1)) \<inter> to_dbltn e"
-      "y \<in> to_dbltn e \<inter> hd (map to_dbltn (C2 @ C1 @ [e] @ C2))" 
-       by(subst (asm) append_butlast_last_id, simp) force
-     have C1C2_empt:"C2@C1 \<noteq> []" 
-       using C1C2 C_prop(3) by force
-     define d1 where "d1 = last (C1 @ [e] @ C2 @ C1)"
-     have d1_def': "d1 = last (C2@C1)"
-       using C1C2_empt d1_def by auto
-     define d2 where "d2 = hd  (C2 @ C1 @ [e] @ C2)"
-     have d2_def': "d2 = hd (C2@C1)" 
-       using C1C2_empt  by(auto simp add: d2_def hd_append)
-     have xy_prop':"x \<in> to_dbltn d1 \<inter> to_dbltn e"
-                   "y \<in> to_dbltn e \<inter> to_dbltn d2" 
-       using xy_prop(5,6)
-       by(all \<open>subst (asm) last_map, simp\<close>, all \<open>subst (asm) hd_map, simp\<close>)
-          (auto simp add: d2_def d1_def)
-     have last_in:"d1 \<in> set C"
-       using C1C2   by(subst d1_def, intro set_rev_mp[OF last_in_set,of _  "set C"]) auto
-     have hd_in:"d2 \<in> set C"
-       using C1C2   by(subst d2_def, intro set_rev_mp[OF hd_in_set,of _  "set C"]) auto
-     have  d1_prop:"d1 \<in> set C" "to_dbltn e \<inter> to_dbltn d1 \<noteq> {}" 
-       using last_in xy_prop(1,5) by(all \<open>subst (asm) last_map, simp\<close>)(auto simp add: d1_def)
-     have  d2_prop:"d2 \<in> set C" "to_dbltn e \<inter> to_dbltn d2 \<noteq> {}" 
-       using hd_in xy_prop(1,6) by(all \<open>subst (asm) hd_map, simp\<close>)(auto simp add: d2_def)
-     have "d1 \<in> insert e (t_set S)" 
-       using C_prop(2) last_in by blast
-     moreover  have d1_not_e:"d1 \<noteq> e"
-     proof(rule ccontr, goal_cases)
-       case 1
-       hence "e \<in> set (C2@C1)"
-         using C1C2_empt d1_def' last_in_set by blast
-       hence "\<not> distinct C"
-         using C1C2 by fastforce
-       then show ?case
-         by (simp add: C_prop(4))
-     qed
-     ultimately have d1_in_S:"d1 \<in>  (t_set S)" 
-       by simp
-     have  "d2 \<in> insert e (t_set S)" 
-       using C_prop(2) hd_in by blast
-     moreover have d2_not_e:"d2 \<noteq> e"
-     proof(rule ccontr, goal_cases)
-       case 1
-       hence "e \<in> set (C2@C1)"
-         using C1C2_empt d2_def' hd_in_set by blast
-       hence "\<not> distinct C"
-         using C1C2 by fastforce
-       then show ?case
-         by (simp add: C_prop(4))
-     qed
-     ultimately have d2_in_S: "d2 \<in> (t_set S)" by simp
+          using epath_find_splitter_advanced[OF e_path_very_verbose] by simp
+        then obtain x y where xy_prop:"to_dbltn e = {x, y}"
+          "x \<noteq> y"
+          "epath (to_dbltn ` insert e (t_set S)) u (map to_dbltn (C1 @ [e] @ C2 @ C1)) x"
+          "epath (to_dbltn ` insert e (t_set S)) y (map to_dbltn (C2 @ C1 @ [e] @ C2)) u"
+          "x \<in> last (map to_dbltn (C1 @ [e] @ C2 @ C1)) \<inter> to_dbltn e"
+          "y \<in> to_dbltn e \<inter> hd (map to_dbltn (C2 @ C1 @ [e] @ C2))" 
+          by(subst (asm) append_butlast_last_id, simp) force
+        have C1C2_empt:"C2@C1 \<noteq> []" 
+          using C1C2 C_prop(3) by force
+        define d1 where "d1 = last (C1 @ [e] @ C2 @ C1)"
+        have d1_def': "d1 = last (C2@C1)"
+          using C1C2_empt d1_def by auto
+        define d2 where "d2 = hd  (C2 @ C1 @ [e] @ C2)"
+        have d2_def': "d2 = hd (C2@C1)" 
+          using C1C2_empt  by(auto simp add: d2_def hd_append)
+        have xy_prop':"x \<in> to_dbltn d1 \<inter> to_dbltn e"
+          "y \<in> to_dbltn e \<inter> to_dbltn d2" 
+          using xy_prop(5,6)
+          by(all \<open>subst (asm) last_map, simp\<close>, all \<open>subst (asm) hd_map, simp\<close>)
+            (auto simp add: d2_def d1_def)
+        have last_in:"d1 \<in> set C"
+          using C1C2   by(subst d1_def, intro set_rev_mp[OF last_in_set,of _  "set C"]) auto
+        have hd_in:"d2 \<in> set C"
+          using C1C2   by(subst d2_def, intro set_rev_mp[OF hd_in_set,of _  "set C"]) auto
+        have  d1_prop:"d1 \<in> set C" "to_dbltn e \<inter> to_dbltn d1 \<noteq> {}" 
+          using last_in xy_prop(1,5) by(all \<open>subst (asm) last_map, simp\<close>)(auto simp add: d1_def)
+        have  d2_prop:"d2 \<in> set C" "to_dbltn e \<inter> to_dbltn d2 \<noteq> {}" 
+          using hd_in xy_prop(1,6) by(all \<open>subst (asm) hd_map, simp\<close>)(auto simp add: d2_def)
+        have "d1 \<in> insert e (t_set S)" 
+          using C_prop(2) last_in by blast
+        moreover  have d1_not_e:"d1 \<noteq> e"
+        proof(rule ccontr, goal_cases)
+          case 1
+          hence "e \<in> set (C2@C1)"
+            using C1C2_empt d1_def' last_in_set by blast
+          hence "\<not> distinct C"
+            using C1C2 by fastforce
+          then show ?case
+            by (simp add: C_prop(4))
+        qed
+        ultimately have d1_in_S:"d1 \<in>  (t_set S)" 
+          by simp
+        have  "d2 \<in> insert e (t_set S)" 
+          using C_prop(2) hd_in by blast
+        moreover have d2_not_e:"d2 \<noteq> e"
+        proof(rule ccontr, goal_cases)
+          case 1
+          hence "e \<in> set (C2@C1)"
+            using C1C2_empt d2_def' hd_in_set by blast
+          hence "\<not> distinct C"
+            using C1C2 by fastforce
+          then show ?case
+            by (simp add: C_prop(4))
+        qed
+        ultimately have d2_in_S: "d2 \<in> (t_set S)" by simp
 
-     have dir_ds_in:"(v1_of d1, v2_of d1) \<in> G.digraph_abs (local.Kruskal_E_to_G S)"
+        have dir_ds_in:"(v1_of d1, v2_of d1) \<in> G.digraph_abs (local.Kruskal_E_to_G S)"
           "(v2_of d1, v1_of d1) \<in> G.digraph_abs (local.Kruskal_E_to_G S)"
           "(v1_of d2, v2_of d2) \<in> G.digraph_abs (local.Kruskal_E_to_G S)"
           "(v2_of d2, v1_of d2) \<in> G.digraph_abs (local.Kruskal_E_to_G S)"
-       by (simp add: d1_in_S d2_in_S digraph_abs_is)+
-     have graph_inv:"G.graph_inv (local.Kruskal_E_to_G S)" 
-       using local.Kruskal_E_to_G_def pair_graph_u_invar by force
-     have "lookup (local.Kruskal_E_to_G S) (v1_of e) \<noteq> None" 
-       using dir_ds_in  d1_prop(2) d2_prop(2) 2 d1_not_e d2_not_e  C1C2_empt  isin.simps(1)  xy_prop(1) xy_prop' 
-       apply(cases "lookup (local.Kruskal_E_to_G S) (v1_of d1)")
-       apply(all \<open>cases "lookup (local.Kruskal_E_to_G S) (v2_of d1)"\<close>)
-       apply(all \<open>cases "lookup (local.Kruskal_E_to_G S) (v1_of d2)"\<close>)
-       apply(all \<open>cases "lookup (local.Kruskal_E_to_G S) (v2_of d2)"\<close>)
-       apply(simp add: doubleton_eq_iff  G.neighbourhood_def Pair_Graph_RBT.G.are_connected_abs[OF graph_inv, symmetric])+
-       by metis
-     moreover have "lookup (local.Kruskal_E_to_G S) (v2_of e) \<noteq> None"
-       using dir_ds_in  d1_prop(2) d2_prop(2) 2 d1_not_e d2_not_e  C1C2_empt  isin.simps(1)  xy_prop(1) xy_prop' 
-       apply(cases "lookup (local.Kruskal_E_to_G S) (v1_of d1)")
-       apply(all \<open>cases "lookup (local.Kruskal_E_to_G S) (v2_of d1)"\<close>)
-       apply(all \<open>cases "lookup (local.Kruskal_E_to_G S) (v1_of d2)"\<close>)
-       apply(all \<open>cases "lookup (local.Kruskal_E_to_G S) (v2_of d2)"\<close>)
-       apply(simp add: doubleton_eq_iff  G.neighbourhood_def Pair_Graph_RBT.G.are_connected_abs[OF graph_inv, symmetric])+
-       by metis+
-     ultimately show ?case
-       using "2" by auto
-   qed
-   thus ?case 
-     using "2" by blast
- qed
-qed
+          by (simp add: d1_in_S d2_in_S digraph_abs_is)+
+        have graph_inv:"G.graph_inv (local.Kruskal_E_to_G S)" 
+          using local.Kruskal_E_to_G_def pair_graph_u_invar by force
+        have "lookup (local.Kruskal_E_to_G S) (v1_of e) \<noteq> None" 
+          using dir_ds_in  d1_prop(2) d2_prop(2) 2 d1_not_e d2_not_e  C1C2_empt  isin.simps(1)  xy_prop(1) xy_prop' 
+          apply(cases "lookup (local.Kruskal_E_to_G S) (v1_of d1)")
+          apply(all \<open>cases "lookup (local.Kruskal_E_to_G S) (v2_of d1)"\<close>)
+          apply(all \<open>cases "lookup (local.Kruskal_E_to_G S) (v1_of d2)"\<close>)
+          apply(all \<open>cases "lookup (local.Kruskal_E_to_G S) (v2_of d2)"\<close>)
+          apply(simp add: doubleton_eq_iff  G.neighbourhood_def Pair_Graph_RBT.G.are_connected_abs[OF graph_inv, symmetric])+
+          by metis
+        moreover have "lookup (local.Kruskal_E_to_G S) (v2_of e) \<noteq> None"
+          using dir_ds_in  d1_prop(2) d2_prop(2) 2 d1_not_e d2_not_e  C1C2_empt  isin.simps(1)  xy_prop(1) xy_prop' 
+          apply(cases "lookup (local.Kruskal_E_to_G S) (v1_of d1)")
+          apply(all \<open>cases "lookup (local.Kruskal_E_to_G S) (v2_of d1)"\<close>)
+          apply(all \<open>cases "lookup (local.Kruskal_E_to_G S) (v1_of d2)"\<close>)
+          apply(all \<open>cases "lookup (local.Kruskal_E_to_G S) (v2_of d2)"\<close>)
+          apply(simp add: doubleton_eq_iff  G.neighbourhood_def Pair_Graph_RBT.G.are_connected_abs[OF graph_inv, symmetric])+
+          by metis+
+        ultimately show ?case
+          using "2" by auto
+      qed
+      thus ?case 
+        using "2" by blast
+    qed
+  qed
   show ?case 
     using second_eq dfs.Graph.vset.set.set_insert[OF assms(1)]
-    by (cases "rbt_subseteq (vset_insert e S) input_G ", 
-       unfold local_indep_oracle_def undirected_multigraph_spec.has_no_cycle_multi_def first_eq ) 
-       auto
+    by (cases "Card_Set2_RBT.subseteq (vset_insert e S) input_G ", 
+        unfold local_indep_oracle_def undirected_multigraph_spec.has_no_cycle_multi_def first_eq ) 
+      auto
 qed
 
 context fixes c::"'e \<Rightarrow> rat" and  order::"'e list"
   assumes non_negative_c:"\<And> e. e \<in> t_set input_G \<Longrightarrow> c e \<ge> 0"
-and order_is_G: "t_set input_G = set order"
-and order_length_is_G_card: "distinct order"
+    and order_is_G: "t_set input_G = set order"
+    and order_length_is_G_card: "distinct order"
 begin
 
-lemma best_in_greedy_axioms:"Best_In_Greedy.BestInGreedy_axioms vset_inv t_set set_of_sets_isin input_G
+lemma best_in_greedy_axioms:"Best_In_Greedy.BestInGreedy_axioms vset_inv t_set input_G
      (Kruskal_Greedy2.indep_graph_matroid v1_of v2_of input_G)"
-    by(auto simp add:  Matroid_Specs_Inst.invar_def local.indep_graph_matroid_def set_of_sets_isin_def
-      Best_In_Greedy.BestInGreedy_axioms_def[OF Kruskal_Greedy2.Kruskal_Greedy.Best_In_Greedy_axioms] G_good Kruskal_Greedy2.indep_graph_matroid_def Matroid_Specs_Inst.indep_def
+  by(auto simp add:  Matroid_Specs_Inst.invar_def local.indep_graph_matroid_def
+      Best_In_Greedy.BestInGreedy_axioms_def[OF Kruskal_Greedy2.Kruskal_Greedy.Best_In_Greedy_axioms] G_good Kruskal_Greedy2.indep_graph_matroid_def
       Matroid_Specs_Inst.finite_setsI)
 
 lemma sort_desc_axioms: "Best_In_Greedy.sort_desc_axioms Kruskal_Greedy.carrier_sorted"
   by (simp add: Kruskal_Greedy.sort_desc_axioms_def insort_key_desc_stable
- length_insort_key_desc set_insort_key_desc sorted_desc_f_insort_key_desc)
+      length_insort_key_desc set_insort_key_desc sorted_desc_f_insort_key_desc)
 
 lemma indep_system_axioms:"Matroid_Specs_Inst.indep_system_axioms input_G
              (Kruskal_Greedy2.indep_graph_matroid v1_of v2_of input_G)"
@@ -859,27 +841,25 @@ lemma indep_system_axioms:"Matroid_Specs_Inst.indep_system_axioms input_G
 proof(rule conjI[OF _ conjI], goal_cases)
   case 1
   then show ?case 
-  by(simp add: rbt_subseteq_correct[OF _ G_good, symmetric]
-           Matroid_Specs_Inst.indep_def Kruskal_Greedy2.indep_graph_matroid_def
-             indep_graph_matroid_def undirected_multigraph.has_no_cycle_multi_def
-             set_of_sets_isin_def) 
+    by(simp add: Card_Set2_RBT.set_subseteq[OF _ G_good, symmetric]
+        Kruskal_Greedy2.indep_graph_matroid_def
+        indep_graph_matroid_def undirected_multigraph.has_no_cycle_multi_def) 
 next
   case 2
   show ?case
     using undirected_multigraph.empty_has_no_cycle_multi_indep 
     by(auto intro!: exI[of _ Leaf] 
-         simp add: Kruskal_Greedy.wrapper_axioms(5) Matroid_Specs_Inst.indep_def 
-                   Kruskal_Greedy2.indep_graph_matroid_def indep_graph_matroid_def set_of_sets_isin_def
-                    local.undirected_multigraph.empty_has_no_cycle_multi_indep)
+        simp add: Kruskal_Greedy.wrapper_axioms(5) 
+        Kruskal_Greedy2.indep_graph_matroid_def indep_graph_matroid_def 
+        local.undirected_multigraph.empty_has_no_cycle_multi_indep)
 next
   case 3
   show ?case
-    unfolding Matroid_Specs_Inst.indep_def Kruskal_Greedy2.indep_graph_matroid_def indep_graph_matroid_def
-              set_of_sets_isin_def
+    unfolding Kruskal_Greedy2.indep_graph_matroid_def indep_graph_matroid_def
   proof(rule+, goal_cases)
     case (1 X Y)
     show ?case 
-      using 1(1,2,4) Custom_Set_RBT.set_subseteq 
+      using 1(1,2,4) Card_Set2_RBT.set_subseteq 
       by (auto intro:  undirected_multigraph.has_no_cycle_multi_indep_subset[OF 1(3)])
   qed
 qed
@@ -892,12 +872,12 @@ lemma size_G_length_order:"size input_G = length order"
 
 lemma valid_order: "Kruskal_Greedy.valid_order input_G order"
   by(simp add: Kruskal_Greedy.valid_order_def Pair_Graph_RBT.set.set_isin G_good  non_negative_c 
-                  size_G_length_order order_is_G)
+      size_G_length_order order_is_G)
 
 lemma kruskal_impl_corespondence: 
   "to_ordinary (kruskal' v1_of v2_of input_G (kruskal_init' c order)) =
   kruskal v1_of v2_of input_G (kruskal_init c order)"
-proof(rule Kruskal_Greedy.BestInGreedy'_corresp, goal_cases)
+proof((subst kruskal_def, subst indep'_def[symmetric]), rule Kruskal_Greedy.BestInGreedy'_corresp, goal_cases)
   case (1 S x)
   then show ?case 
     by(unfold Kruskal_Greedy2.local_indep_oracle_def, intro local_indep_oracle_correct) auto
@@ -908,7 +888,7 @@ next
 next
   case 3
   then show ?case
-    by (simp add: best_in_greedy_axioms) 
+    by (simp add: best_in_greedy_axioms indep'_def)
 next
   case 4
   then show ?case 
@@ -916,7 +896,7 @@ next
 next
   case 5
   then show ?case
-    by (simp add: indep_system_axioms)
+    by (simp add: indep_system_axioms indep'_def)
 next
   case 6
   then show ?case
@@ -929,7 +909,7 @@ qed
 
 lemma indep_finite: "undirected_multigraph_spec.has_no_cycle_multi to_dbltn (t_set input_G) X \<Longrightarrow> finite X"
   using Spanning_Trees.undirected_multigraph.graph_indep_system_multi indep_system.indep_finite
- undirected_multigraph.undirected_multigraph_axioms by fast
+    undirected_multigraph.undirected_multigraph_axioms by fast
 
 lemma idnep_in_G:"undirected_multigraph_spec.has_no_cycle_multi to_dbltn (t_set input_G) X \<Longrightarrow>
            x \<in> X \<Longrightarrow> x \<in> t_set input_G"
@@ -939,26 +919,26 @@ lemma indep_system_order:"indep_system (set order) (undirected_multigraph_spec.h
   using local.undirected_multigraph.graph_indep_system_multi[of input_G] order_is_G by auto
 
 interpretation use_greedy_thms_kruskal:
-Use_Greedy_Thms Leaf vset_insert vset_delete isin t_set vset_inv vset_union
-                               vset_inter vset_diff rbt_subseteq  size set_of_sets_isin 
-"undirected_multigraph_spec.has_no_cycle_multi (\<lambda> e. {v1_of e, v2_of e})(Tree2.set_tree input_G)"
-input_G c order Kruskal_Greedy.carrier_sorted
+  Use_Greedy_Thms Leaf vset_insert vset_delete isin t_set vset_inv vset_union
+  vset_inter vset_diff  size  
+  "undirected_multigraph_spec.has_no_cycle_multi (\<lambda> e. {v1_of e, v2_of e})(Tree2.set_tree input_G)"
+  input_G c order Kruskal_Greedy.carrier_sorted
   by(intro Use_Greedy_Thms.intro 
-                      undirected_multigraph.graph_indep_system_multi indep_finite idnep_in_G)
+      undirected_multigraph.graph_indep_system_multi indep_finite idnep_in_G)
     (auto intro!: Use_Greedy_Thms_axioms.intro
-       simp add: Matroid_Specs_Inst.Matroid_Specs_axioms[simplified Matroid_Specs_def]
-                       set_of_sets_isin_def' G_good non_negative_c order_is_G
-                      indep_system_order indep_finite undirected_multigraph_spec.has_no_cycle_multi_def
-                      order_length_is_G_card sort_desc_axioms)
+      simp add: Matroid_Specs_Inst.Matroid_Specs_axioms[simplified Matroid_Specs_def]
+      G_good non_negative_c order_is_G
+      indep_system_order indep_finite undirected_multigraph_spec.has_no_cycle_multi_def
+      order_length_is_G_card sort_desc_axioms)
 
 lemma kruskal_returns_basis: "indep_system.basis (t_set input_G) 
 (undirected_multigraph_spec.has_no_cycle_multi to_dbltn (t_set input_G))
  (t_set (result (kruskal v1_of v2_of input_G (kruskal_init c order))))"
   by(simp add:  kruskal_def Kruskal_Greedy2.indep_graph_matroid_def local.indep_graph_matroid_def 
-                kruskal_init_def use_greedy_thms_kruskal.algo_gives_basis )
+      kruskal_init_def use_greedy_thms_kruskal.algo_gives_basis )
 
 corollary kruskal_returns_spanning_forest: 
-"undirected_multigraph_spec.is_spanning_forest_multi to_dbltn (t_set input_G)
+  "undirected_multigraph_spec.is_spanning_forest_multi to_dbltn (t_set input_G)
  (t_set (result (kruskal v1_of v2_of input_G (kruskal_init c order))))"
   apply(subst undirected_multigraph.spanning_forest_iff_basis_multi)
   by(rule kruskal_returns_basis)
@@ -967,13 +947,13 @@ lemma rank_quotient_one: "indep_system.rank_quotient (t_set input_G)
     (undirected_multigraph_spec.has_no_cycle_multi to_dbltn (t_set input_G)) = 1"
   apply(subst Matroids_Theory.indep_system.matroid_iff_rq_eq_1[symmetric])
   by (auto simp add: use_greedy_thms_kruskal.indep_system 
-                undirected_multigraph.graph_matroid_multi)
+      undirected_multigraph.graph_matroid_multi)
 
 theorem kruskal_is_max:
-"undirected_multigraph_spec.has_no_cycle_multi to_dbltn (t_set input_G) X \<Longrightarrow>
+  "undirected_multigraph_spec.has_no_cycle_multi to_dbltn (t_set input_G) X \<Longrightarrow>
 sum c X \<le> sum c (t_set (result (kruskal v1_of v2_of input_G (kruskal_init c order))))"
   unfolding kruskal_def kruskal_init_def Kruskal_Greedy2.indep_graph_matroid_def
-            local.indep_graph_matroid_def
+    local.indep_graph_matroid_def
   apply(rule order.trans[rotated])
   apply(rule use_greedy_thms_kruskal.indep_predicate_greedy_correct[of X])
   by(simp add:  rank_quotient_one)+
@@ -984,7 +964,7 @@ definition "max_forest X =
      sum c Y \<le> sum c X))"
 
 corollary kruskal_computes_max_spanning_forest:
-"max_forest(t_set (result (kruskal v1_of v2_of input_G (kruskal_init c order))))"
+  "max_forest(t_set (result (kruskal v1_of v2_of input_G (kruskal_init c order))))"
   using kruskal_is_max kruskal_returns_spanning_forest 
   by(auto simp add: max_forest_def undirected_multigraph.is_spanning_forest_multi_def)
 end
@@ -1004,14 +984,14 @@ qed
 
 
 definition "edges = [(0::nat, 1::nat), (0, 2), (2, 3), (2,4), (2,1), (1,5), (5,8), (8,7), (7,1),
-                     (7,2), (7,4), (4,3), (3,4), (3,3), (9, 8), (8, 1), (4,5), (5,10)]"
+                     (7,2), (7,4), (4,3), (3,4), (3,3), (9, 8), (8, 1), (4,5), (5,10), (10,5), (10,1)]"
 
 definition "G = foldr (\<lambda> x tree. vset_insert x  tree) edges empty"
 
 definition "c_list = [((0::nat, 1::nat), 1::rat), ((0, 2), 0.5), ((2, 3), 5/8), ((2,4), 3), ((2,1), -1/3),
                       ((1,5), 4), ((5,8), 2), ((8,7), 0.1), ((7,1), 1.3),
                      ((7,2), 3), ((7,4), 3), ((4,3), 2), ((3,4), 1), ((3,3), 0), ((9, 8),2.5),
-                      ((8, 1), 0), ((4,5), 2), ((5,10), 3)]"
+                      ((8, 1), 0), ((4,5), 2), ((5,10), 3), ((10,5), 30), ((10,1), 1000)]"
 
 definition "c_impl = foldr (\<lambda> xy tree. update (prod.fst xy) (prod.snd xy) tree) c_list Leaf"
 value "c_impl"
